2/new_folder2/corral_out.bpl
@@ -4,7 +4,7 @@ type ContractName;
 
 const unique null: Ref;
 
-const unique SimpleMarketplace: ContractName;
+const unique AssetTransfer: ContractName;
 
 function ConstantToRef(x: int) : Ref;
 
@@ -31,10 +31,6 @@ var DType: [Ref]ContractName;
 var Alloc: [Ref]bool;
 
 var balance_ADDR: [Ref]int;
-
-var M_int_int: [Ref][int]int;
-
-var M_int_Ref: [Ref][int]Ref;
 
 var Length: [Ref]int;
 
@@ -90,12 +86,11 @@ axiom (forall __i__0_0: Ref, __i__0_1: Ref :: { abiEncodePacked1R(__i__0_0), abi
 
 axiom (forall __i__0_0: Ref, __i__0_1: Ref, __i__1_0: int, __i__1_1: int :: { abiEncodePacked2R(__i__0_0, __i__1_0), abiEncodePacked2R(__i__0_1, __i__1_1) } (__i__0_0 == __i__0_1 && __i__1_0 == __i__1_1) || abiEncodePacked2R(__i__0_0, __i__1_0) != abiEncodePacked2R(__i__0_1, __i__1_1));
 
-procedure {:public} prueba_SimpleMarketplace(this: Ref, msgsender_MSG: Ref, msgvalue_MSG: int, offerPrice_s60: int);
-  modifies StateEnum_SimpleMarketplace;
+procedure {:public} prueba_AssetTransfer(this: Ref, msgsender_MSG: Ref, msgvalue_MSG: int, offerPrice_s135: int, inspector_s135: Ref, appraiser_s135: Ref, description_s135: int, price_s135: int);
 
 
 
-implementation {:ForceInline} prueba_SimpleMarketplace(this: Ref, msgsender_MSG: Ref, msgvalue_MSG: int, offerPrice_s60: int)
+implementation {:ForceInline} prueba_AssetTransfer(this: Ref, msgsender_MSG: Ref, msgvalue_MSG: int, offerPrice_s135: int, inspector_s135: Ref, appraiser_s135: Ref, description_s135: int, price_s135: int)
 {
 
   anon0:
@@ -103,131 +98,126 @@ implementation {:ForceInline} prueba_SimpleMarketplace(this: Ref, msgsender_MSG:
     call {:si_unique_call 1} {:cexpr "this"} boogie_si_record_sol2Bpl_ref(this);
     call {:si_unique_call 2} {:cexpr "msg.sender"} boogie_si_record_sol2Bpl_ref(msgsender_MSG);
     call {:si_unique_call 3} {:cexpr "msg.value"} boogie_si_record_sol2Bpl_int(msgvalue_MSG);
-    call {:si_unique_call 4} {:cexpr "offerPrice"} boogie_si_record_sol2Bpl_int(offerPrice_s60);
-    call {:si_unique_call 5} {:cexpr "_verisolLastArg"} boogie_si_record_sol2Bpl_bool(true);
+    call {:si_unique_call 4} {:cexpr "offerPrice"} boogie_si_record_sol2Bpl_int(offerPrice_s135);
+    call {:si_unique_call 5} {:cexpr "inspector"} boogie_si_record_sol2Bpl_ref(inspector_s135);
+    call {:si_unique_call 6} {:cexpr "appraiser"} boogie_si_record_sol2Bpl_ref(appraiser_s135);
+    call {:si_unique_call 7} {:cexpr "description"} boogie_si_record_sol2Bpl_int(description_s135);
+    call {:si_unique_call 8} {:cexpr "price"} boogie_si_record_sol2Bpl_int(price_s135);
+    call {:si_unique_call 9} {:cexpr "_verisolLastArg"} boogie_si_record_sol2Bpl_bool(true);
     goto corral_source_split_1;
 
   corral_source_split_1:
     goto corral_source_split_2;
 
   corral_source_split_2:
-    assume !(StateEnum_SimpleMarketplace[this] == 0) && StateEnum_SimpleMarketplace[this] == 1 && StateEnum_SimpleMarketplace[this] == 1;
+    assume !(State_AssetTransfer[this] == 0) && !(State_AssetTransfer[this] == 0) && !(State_AssetTransfer[this] == 1) && !(State_AssetTransfer[this] == 1 || State_AssetTransfer[this] == 2 || State_AssetTransfer[this] == 3 || (State_AssetTransfer[this] == 4 && State_AssetTransfer[this] == 5) || State_AssetTransfer[this] == 6) && !(State_AssetTransfer[this] == 1) && (State_AssetTransfer[this] == 1 || State_AssetTransfer[this] == 2 || State_AssetTransfer[this] == 3 || State_AssetTransfer[this] == 4 || State_AssetTransfer[this] == 5 || State_AssetTransfer[this] == 7) && (State_AssetTransfer[this] != 2 || State_AssetTransfer[this] != 3) && (State_AssetTransfer[this] != 2 || State_AssetTransfer[this] != 4);
     goto corral_source_split_3;
 
   corral_source_split_3:
-    assume msgsender_MSG == InstanceOwner_SimpleMarketplace[this];
-    goto corral_source_split_4;
-
-  corral_source_split_4:
-    call {:si_unique_call 6} Reject_SimpleMarketplace(this, msgsender_MSG, msgvalue_MSG);
-    goto corral_source_split_5;
-
-  corral_source_split_5:
-    assert !(StateEnum_SimpleMarketplace[this] == 0 && !(StateEnum_SimpleMarketplace[this] == 1) && !(StateEnum_SimpleMarketplace[this] == 1));
+    assert false;
     return;
 }
 
 
 
-var InstanceOwner_SimpleMarketplace: [Ref]Ref;
+var InstanceOwner_AssetTransfer: [Ref]Ref;
 
-var Description_SimpleMarketplace: [Ref]int;
+var Description_AssetTransfer: [Ref]int;
 
-var AskingPrice_SimpleMarketplace: [Ref]int;
+var AskingPrice_AssetTransfer: [Ref]int;
 
-var StateEnum_SimpleMarketplace: [Ref]int;
+var State_AssetTransfer: [Ref]int;
 
-var result_SimpleMarketplace: [Ref]Ref;
+var InstanceBuyer_AssetTransfer: [Ref]Ref;
 
-var InstanceBuyer_SimpleMarketplace: [Ref]Ref;
+var OfferPrice_AssetTransfer: [Ref]int;
 
-var OfferPrice_SimpleMarketplace: [Ref]int;
+var InstanceInspector_AssetTransfer: [Ref]Ref;
 
-procedure SimpleMarketplace_SimpleMarketplace_NoBaseCtor(this: Ref, msgsender_MSG: Ref, msgvalue_MSG: int, description_s107: int, price_s107: int, sender_s107: Ref);
-  modifies Balance, InstanceOwner_SimpleMarketplace, Description_SimpleMarketplace, AskingPrice_SimpleMarketplace, Alloc, result_SimpleMarketplace, InstanceBuyer_SimpleMarketplace, OfferPrice_SimpleMarketplace, StateEnum_SimpleMarketplace;
+var InstanceAppraiser_AssetTransfer: [Ref]Ref;
+
+procedure AssetTransfer_AssetTransfer_NoBaseCtor(this: Ref, msgsender_MSG: Ref, msgvalue_MSG: int, description_s188: int, price_s188: int);
+  modifies Balance, InstanceOwner_AssetTransfer, Description_AssetTransfer, AskingPrice_AssetTransfer, InstanceBuyer_AssetTransfer, OfferPrice_AssetTransfer, InstanceInspector_AssetTransfer, InstanceAppraiser_AssetTransfer, State_AssetTransfer;
 
 
 
-implementation {:ForceInline} SimpleMarketplace_SimpleMarketplace_NoBaseCtor(this: Ref, msgsender_MSG: Ref, msgvalue_MSG: int, description_s107: int, price_s107: int, sender_s107: Ref)
+implementation {:ForceInline} AssetTransfer_AssetTransfer_NoBaseCtor(this: Ref, msgsender_MSG: Ref, msgvalue_MSG: int, description_s188: int, price_s188: int)
 {
-  var __var_1: Ref;
 
   anon0:
     assume msgsender_MSG != null;
     Balance[this] := 0;
-    InstanceOwner_SimpleMarketplace[this] := null;
-    Description_SimpleMarketplace[this] := -989211026;
-    AskingPrice_SimpleMarketplace[this] := 0;
-    call {:si_unique_call 7} __var_1 := FreshRefGenerator();
-    result_SimpleMarketplace[this] := __var_1;
-    assume Length[result_SimpleMarketplace[this]] == 0;
-    InstanceBuyer_SimpleMarketplace[this] := null;
-    OfferPrice_SimpleMarketplace[this] := 0;
-    call {:si_unique_call 8} {:cexpr "_verisolFirstArg"} boogie_si_record_sol2Bpl_bool(false);
-    call {:si_unique_call 9} {:cexpr "this"} boogie_si_record_sol2Bpl_ref(this);
-    call {:si_unique_call 10} {:cexpr "msg.sender"} boogie_si_record_sol2Bpl_ref(msgsender_MSG);
-    call {:si_unique_call 11} {:cexpr "msg.value"} boogie_si_record_sol2Bpl_int(msgvalue_MSG);
-    call {:si_unique_call 12} {:cexpr "description"} boogie_si_record_sol2Bpl_int(description_s107);
-    call {:si_unique_call 13} {:cexpr "price"} boogie_si_record_sol2Bpl_int(price_s107);
-    call {:si_unique_call 14} {:cexpr "sender"} boogie_si_record_sol2Bpl_ref(sender_s107);
-    call {:si_unique_call 15} {:cexpr "_verisolLastArg"} boogie_si_record_sol2Bpl_bool(true);
+    InstanceOwner_AssetTransfer[this] := null;
+    Description_AssetTransfer[this] := -111333532;
+    AskingPrice_AssetTransfer[this] := 0;
+    InstanceBuyer_AssetTransfer[this] := null;
+    OfferPrice_AssetTransfer[this] := 0;
+    InstanceInspector_AssetTransfer[this] := null;
+    InstanceAppraiser_AssetTransfer[this] := null;
+    call {:si_unique_call 10} {:cexpr "_verisolFirstArg"} boogie_si_record_sol2Bpl_bool(false);
+    call {:si_unique_call 11} {:cexpr "this"} boogie_si_record_sol2Bpl_ref(this);
+    call {:si_unique_call 12} {:cexpr "msg.sender"} boogie_si_record_sol2Bpl_ref(msgsender_MSG);
+    call {:si_unique_call 13} {:cexpr "msg.value"} boogie_si_record_sol2Bpl_int(msgvalue_MSG);
+    call {:si_unique_call 14} {:cexpr "description"} boogie_si_record_sol2Bpl_int(description_s188);
+    call {:si_unique_call 15} {:cexpr "price"} boogie_si_record_sol2Bpl_int(price_s188);
+    call {:si_unique_call 16} {:cexpr "_verisolLastArg"} boogie_si_record_sol2Bpl_bool(true);
+    goto corral_source_split_5;
+
+  corral_source_split_5:
+    goto corral_source_split_6;
+
+  corral_source_split_6:
+    InstanceOwner_AssetTransfer[this] := msgsender_MSG;
+    call {:si_unique_call 17} {:cexpr "InstanceOwner"} boogie_si_record_sol2Bpl_ref(InstanceOwner_AssetTransfer[this]);
     goto corral_source_split_7;
 
   corral_source_split_7:
+    assume AskingPrice_AssetTransfer[this] >= 0;
+    assume price_s188 >= 0;
+    AskingPrice_AssetTransfer[this] := price_s188;
+    call {:si_unique_call 18} {:cexpr "AskingPrice"} boogie_si_record_sol2Bpl_int(AskingPrice_AssetTransfer[this]);
     goto corral_source_split_8;
 
   corral_source_split_8:
-    InstanceOwner_SimpleMarketplace[this] := sender_s107;
-    call {:si_unique_call 16} {:cexpr "InstanceOwner"} boogie_si_record_sol2Bpl_ref(InstanceOwner_SimpleMarketplace[this]);
+    Description_AssetTransfer[this] := description_s188;
+    call {:si_unique_call 19} {:cexpr "Description"} boogie_si_record_sol2Bpl_int(Description_AssetTransfer[this]);
     goto corral_source_split_9;
 
   corral_source_split_9:
-    AskingPrice_SimpleMarketplace[this] := price_s107;
-    call {:si_unique_call 17} {:cexpr "AskingPrice"} boogie_si_record_sol2Bpl_int(AskingPrice_SimpleMarketplace[this]);
-    goto corral_source_split_10;
-
-  corral_source_split_10:
-    Description_SimpleMarketplace[this] := description_s107;
-    call {:si_unique_call 18} {:cexpr "Description"} boogie_si_record_sol2Bpl_int(Description_SimpleMarketplace[this]);
-    goto corral_source_split_11;
-
-  corral_source_split_11:
-    StateEnum_SimpleMarketplace[this] := 0;
+    State_AssetTransfer[this] := 0;
     return;
 }
 
 
 
-procedure {:constructor} {:public} SimpleMarketplace_SimpleMarketplace(this: Ref, msgsender_MSG: Ref, msgvalue_MSG: int, description_s107: int, price_s107: int, sender_s107: Ref);
-  modifies Balance, InstanceOwner_SimpleMarketplace, Description_SimpleMarketplace, AskingPrice_SimpleMarketplace, Alloc, result_SimpleMarketplace, InstanceBuyer_SimpleMarketplace, OfferPrice_SimpleMarketplace, StateEnum_SimpleMarketplace;
+procedure {:constructor} {:public} AssetTransfer_AssetTransfer(this: Ref, msgsender_MSG: Ref, msgvalue_MSG: int, description_s188: int, price_s188: int);
+  modifies Balance, InstanceOwner_AssetTransfer, Description_AssetTransfer, AskingPrice_AssetTransfer, InstanceBuyer_AssetTransfer, OfferPrice_AssetTransfer, InstanceInspector_AssetTransfer, InstanceAppraiser_AssetTransfer, State_AssetTransfer;
 
 
 
-implementation {:ForceInline} SimpleMarketplace_SimpleMarketplace(this: Ref, msgsender_MSG: Ref, msgvalue_MSG: int, description_s107: int, price_s107: int, sender_s107: Ref)
+implementation {:ForceInline} AssetTransfer_AssetTransfer(this: Ref, msgsender_MSG: Ref, msgvalue_MSG: int, description_s188: int, price_s188: int)
 {
-  var __var_1: Ref;
 
   anon0:
-    call {:si_unique_call 19} {:cexpr "_verisolFirstArg"} boogie_si_record_sol2Bpl_bool(false);
-    call {:si_unique_call 20} {:cexpr "this"} boogie_si_record_sol2Bpl_ref(this);
-    call {:si_unique_call 21} {:cexpr "msg.sender"} boogie_si_record_sol2Bpl_ref(msgsender_MSG);
-    call {:si_unique_call 22} {:cexpr "msg.value"} boogie_si_record_sol2Bpl_int(msgvalue_MSG);
-    call {:si_unique_call 23} {:cexpr "description"} boogie_si_record_sol2Bpl_int(description_s107);
-    call {:si_unique_call 24} {:cexpr "price"} boogie_si_record_sol2Bpl_int(price_s107);
-    call {:si_unique_call 25} {:cexpr "sender"} boogie_si_record_sol2Bpl_ref(sender_s107);
+    call {:si_unique_call 20} {:cexpr "_verisolFirstArg"} boogie_si_record_sol2Bpl_bool(false);
+    call {:si_unique_call 21} {:cexpr "this"} boogie_si_record_sol2Bpl_ref(this);
+    call {:si_unique_call 22} {:cexpr "msg.sender"} boogie_si_record_sol2Bpl_ref(msgsender_MSG);
+    call {:si_unique_call 23} {:cexpr "msg.value"} boogie_si_record_sol2Bpl_int(msgvalue_MSG);
+    call {:si_unique_call 24} {:cexpr "description"} boogie_si_record_sol2Bpl_int(description_s188);
+    call {:si_unique_call 25} {:cexpr "price"} boogie_si_record_sol2Bpl_int(price_s188);
     call {:si_unique_call 26} {:cexpr "_verisolLastArg"} boogie_si_record_sol2Bpl_bool(true);
-    call {:si_unique_call 27} SimpleMarketplace_SimpleMarketplace_NoBaseCtor(this, msgsender_MSG, msgvalue_MSG, description_s107, price_s107, sender_s107);
+    call {:si_unique_call 27} AssetTransfer_AssetTransfer_NoBaseCtor(this, msgsender_MSG, msgvalue_MSG, description_s188, price_s188);
     return;
 }
 
 
 
-procedure {:public} MakeOffer_SimpleMarketplace(this: Ref, msgsender_MSG: Ref, msgvalue_MSG: int, offerPrice_s153: int);
-  modifies InstanceBuyer_SimpleMarketplace, OfferPrice_SimpleMarketplace, StateEnum_SimpleMarketplace;
+procedure {:public} Terminate_AssetTransfer(this: Ref, msgsender_MSG: Ref, msgvalue_MSG: int);
+  modifies State_AssetTransfer;
 
 
 
-implementation {:ForceInline} MakeOffer_SimpleMarketplace(this: Ref, msgsender_MSG: Ref, msgvalue_MSG: int, offerPrice_s153: int)
+implementation {:ForceInline} Terminate_AssetTransfer(this: Ref, msgsender_MSG: Ref, msgvalue_MSG: int)
 {
 
   anon0:
@@ -235,108 +225,141 @@ implementation {:ForceInline} MakeOffer_SimpleMarketplace(this: Ref, msgsender_M
     call {:si_unique_call 29} {:cexpr "this"} boogie_si_record_sol2Bpl_ref(this);
     call {:si_unique_call 30} {:cexpr "msg.sender"} boogie_si_record_sol2Bpl_ref(msgsender_MSG);
     call {:si_unique_call 31} {:cexpr "msg.value"} boogie_si_record_sol2Bpl_int(msgvalue_MSG);
-    call {:si_unique_call 32} {:cexpr "offerPrice"} boogie_si_record_sol2Bpl_int(offerPrice_s153);
-    call {:si_unique_call 33} {:cexpr "_verisolLastArg"} boogie_si_record_sol2Bpl_bool(true);
-    goto corral_source_split_13;
+    call {:si_unique_call 32} {:cexpr "_verisolLastArg"} boogie_si_record_sol2Bpl_bool(true);
+    goto corral_source_split_11;
 
-  corral_source_split_13:
+  corral_source_split_11:
+    goto corral_source_split_12;
+
+  corral_source_split_12:
+    goto anon3_Then, anon3_Else;
+
+  anon3_Then:
+    assume {:partition} InstanceOwner_AssetTransfer[this] != msgsender_MSG;
     goto corral_source_split_14;
 
   corral_source_split_14:
-    goto anon7_Then, anon7_Else;
+    goto corral_source_split_15;
 
-  anon7_Then:
-    assume {:partition} offerPrice_s153 == 0;
-    goto corral_source_split_16;
-
-  corral_source_split_16:
-    goto corral_source_split_17;
-
-  corral_source_split_17:
+  corral_source_split_15:
     assume false;
     goto anon2;
 
-  anon7_Else:
-    assume {:partition} offerPrice_s153 != 0;
+  anon3_Else:
+    assume {:partition} InstanceOwner_AssetTransfer[this] == msgsender_MSG;
     goto anon2;
 
   anon2:
-    goto anon8_Then, anon8_Else;
-
-  anon8_Then:
-    assume {:partition} StateEnum_SimpleMarketplace[this] != 0;
-    goto corral_source_split_19;
-
-  corral_source_split_19:
-    goto corral_source_split_20;
-
-  corral_source_split_20:
-    assume false;
-    goto anon4;
-
-  anon8_Else:
-    assume {:partition} StateEnum_SimpleMarketplace[this] == 0;
-    goto anon4;
-
-  anon4:
-    goto anon9_Then, anon9_Else;
-
-  anon9_Then:
-    assume {:partition} InstanceOwner_SimpleMarketplace[this] == msgsender_MSG;
-    goto corral_source_split_22;
-
-  corral_source_split_22:
-    goto corral_source_split_23;
-
-  corral_source_split_23:
-    assume false;
-    goto anon6;
-
-  anon9_Else:
-    assume {:partition} InstanceOwner_SimpleMarketplace[this] != msgsender_MSG;
-    goto anon6;
-
-  anon6:
-    InstanceBuyer_SimpleMarketplace[this] := msgsender_MSG;
-    call {:si_unique_call 34} {:cexpr "InstanceBuyer"} boogie_si_record_sol2Bpl_ref(InstanceBuyer_SimpleMarketplace[this]);
-    goto corral_source_split_25;
-
-  corral_source_split_25:
-    OfferPrice_SimpleMarketplace[this] := offerPrice_s153;
-    call {:si_unique_call 35} {:cexpr "OfferPrice"} boogie_si_record_sol2Bpl_int(OfferPrice_SimpleMarketplace[this]);
-    goto corral_source_split_26;
-
-  corral_source_split_26:
-    StateEnum_SimpleMarketplace[this] := 1;
+    State_AssetTransfer[this] := 9;
     return;
 }
 
 
 
-procedure {:public} Reject_SimpleMarketplace(this: Ref, msgsender_MSG: Ref, msgvalue_MSG: int);
-  modifies StateEnum_SimpleMarketplace;
+procedure {:public} Modify_AssetTransfer(this: Ref, msgsender_MSG: Ref, msgvalue_MSG: int, description_s240: int, price_s240: int);
+  modifies Description_AssetTransfer, AskingPrice_AssetTransfer;
 
 
 
-implementation {:ForceInline} Reject_SimpleMarketplace(this: Ref, msgsender_MSG: Ref, msgvalue_MSG: int)
+implementation {:ForceInline} Modify_AssetTransfer(this: Ref, msgsender_MSG: Ref, msgvalue_MSG: int, description_s240: int, price_s240: int)
 {
 
   anon0:
-    call {:si_unique_call 36} {:cexpr "_verisolFirstArg"} boogie_si_record_sol2Bpl_bool(false);
-    call {:si_unique_call 37} {:cexpr "this"} boogie_si_record_sol2Bpl_ref(this);
-    call {:si_unique_call 38} {:cexpr "msg.sender"} boogie_si_record_sol2Bpl_ref(msgsender_MSG);
-    call {:si_unique_call 39} {:cexpr "msg.value"} boogie_si_record_sol2Bpl_int(msgvalue_MSG);
-    call {:si_unique_call 40} {:cexpr "_verisolLastArg"} boogie_si_record_sol2Bpl_bool(true);
+    call {:si_unique_call 33} {:cexpr "_verisolFirstArg"} boogie_si_record_sol2Bpl_bool(false);
+    call {:si_unique_call 34} {:cexpr "this"} boogie_si_record_sol2Bpl_ref(this);
+    call {:si_unique_call 35} {:cexpr "msg.sender"} boogie_si_record_sol2Bpl_ref(msgsender_MSG);
+    call {:si_unique_call 36} {:cexpr "msg.value"} boogie_si_record_sol2Bpl_int(msgvalue_MSG);
+    call {:si_unique_call 37} {:cexpr "description"} boogie_si_record_sol2Bpl_int(description_s240);
+    call {:si_unique_call 38} {:cexpr "price"} boogie_si_record_sol2Bpl_int(price_s240);
+    call {:si_unique_call 39} {:cexpr "_verisolLastArg"} boogie_si_record_sol2Bpl_bool(true);
+    goto corral_source_split_17;
+
+  corral_source_split_17:
+    goto corral_source_split_18;
+
+  corral_source_split_18:
+    goto anon5_Then, anon5_Else;
+
+  anon5_Then:
+    assume {:partition} State_AssetTransfer[this] != 0;
+    goto corral_source_split_20;
+
+  corral_source_split_20:
+    goto corral_source_split_21;
+
+  corral_source_split_21:
+    assume false;
+    goto anon2;
+
+  anon5_Else:
+    assume {:partition} State_AssetTransfer[this] == 0;
+    goto anon2;
+
+  anon2:
+    goto anon6_Then, anon6_Else;
+
+  anon6_Then:
+    assume {:partition} InstanceOwner_AssetTransfer[this] != msgsender_MSG;
+    goto corral_source_split_23;
+
+  corral_source_split_23:
+    goto corral_source_split_24;
+
+  corral_source_split_24:
+    assume false;
+    goto anon4;
+
+  anon6_Else:
+    assume {:partition} InstanceOwner_AssetTransfer[this] == msgsender_MSG;
+    goto anon4;
+
+  anon4:
+    Description_AssetTransfer[this] := description_s240;
+    call {:si_unique_call 40} {:cexpr "Description"} boogie_si_record_sol2Bpl_int(Description_AssetTransfer[this]);
+    goto corral_source_split_26;
+
+  corral_source_split_26:
+    assume AskingPrice_AssetTransfer[this] >= 0;
+    assume price_s240 >= 0;
+    AskingPrice_AssetTransfer[this] := price_s240;
+    call {:si_unique_call 41} {:cexpr "AskingPrice"} boogie_si_record_sol2Bpl_int(AskingPrice_AssetTransfer[this]);
+    return;
+}
+
+
+
+procedure {:public} MakeOffer_AssetTransfer(this: Ref, msgsender_MSG: Ref, msgvalue_MSG: int, inspector_s310: Ref, appraiser_s310: Ref, offerPrice_s310: int);
+  modifies InstanceBuyer_AssetTransfer, InstanceInspector_AssetTransfer, InstanceAppraiser_AssetTransfer, OfferPrice_AssetTransfer, State_AssetTransfer;
+
+
+
+implementation {:ForceInline} MakeOffer_AssetTransfer(this: Ref, msgsender_MSG: Ref, msgvalue_MSG: int, inspector_s310: Ref, appraiser_s310: Ref, offerPrice_s310: int)
+{
+  var __var_1: Ref;
+  var __var_2: Ref;
+
+  anon0:
+    call {:si_unique_call 42} {:cexpr "_verisolFirstArg"} boogie_si_record_sol2Bpl_bool(false);
+    call {:si_unique_call 43} {:cexpr "this"} boogie_si_record_sol2Bpl_ref(this);
+    call {:si_unique_call 44} {:cexpr "msg.sender"} boogie_si_record_sol2Bpl_ref(msgsender_MSG);
+    call {:si_unique_call 45} {:cexpr "msg.value"} boogie_si_record_sol2Bpl_int(msgvalue_MSG);
+    call {:si_unique_call 46} {:cexpr "inspector"} boogie_si_record_sol2Bpl_ref(inspector_s310);
+    call {:si_unique_call 47} {:cexpr "appraiser"} boogie_si_record_sol2Bpl_ref(appraiser_s310);
+    call {:si_unique_call 48} {:cexpr "offerPrice"} boogie_si_record_sol2Bpl_int(offerPrice_s310);
+    call {:si_unique_call 49} {:cexpr "_verisolLastArg"} boogie_si_record_sol2Bpl_bool(true);
     goto corral_source_split_28;
 
   corral_source_split_28:
     goto corral_source_split_29;
 
   corral_source_split_29:
-    goto anon5_Then, anon5_Else;
+    __var_1 := null;
+    __var_2 := null;
+    assume offerPrice_s310 >= 0;
+    goto anon7_Then, anon7_Else;
 
-  anon5_Then:
-    assume {:partition} StateEnum_SimpleMarketplace[this] != 1;
+  anon7_Then:
+    assume {:partition} inspector_s310 == null || appraiser_s310 == null || offerPrice_s310 == 0;
     goto corral_source_split_31;
 
   corral_source_split_31:
@@ -346,15 +369,15 @@ implementation {:ForceInline} Reject_SimpleMarketplace(this: Ref, msgsender_MSG:
     assume false;
     goto anon2;
 
-  anon5_Else:
-    assume {:partition} StateEnum_SimpleMarketplace[this] == 1;
+  anon7_Else:
+    assume {:partition} !(inspector_s310 == null || appraiser_s310 == null || offerPrice_s310 == 0);
     goto anon2;
 
   anon2:
-    goto anon6_Then, anon6_Else;
+    goto anon8_Then, anon8_Else;
 
-  anon6_Then:
-    assume {:partition} InstanceOwner_SimpleMarketplace[this] != msgsender_MSG;
+  anon8_Then:
+    assume {:partition} State_AssetTransfer[this] != 0;
     goto corral_source_split_34;
 
   corral_source_split_34:
@@ -364,74 +387,656 @@ implementation {:ForceInline} Reject_SimpleMarketplace(this: Ref, msgsender_MSG:
     assume false;
     goto anon4;
 
-  anon6_Else:
-    assume {:partition} InstanceOwner_SimpleMarketplace[this] == msgsender_MSG;
+  anon8_Else:
+    assume {:partition} State_AssetTransfer[this] == 0;
     goto anon4;
 
   anon4:
-    StateEnum_SimpleMarketplace[this] := 0;
-    return;
-}
+    goto anon9_Then, anon9_Else;
 
-
-
-procedure {:public} AcceptOffer_SimpleMarketplace(this: Ref, msgsender_MSG: Ref, msgvalue_MSG: int);
-  modifies StateEnum_SimpleMarketplace;
-
-
-
-implementation {:ForceInline} AcceptOffer_SimpleMarketplace(this: Ref, msgsender_MSG: Ref, msgvalue_MSG: int)
-{
-
-  anon0:
-    call {:si_unique_call 41} {:cexpr "_verisolFirstArg"} boogie_si_record_sol2Bpl_bool(false);
-    call {:si_unique_call 42} {:cexpr "this"} boogie_si_record_sol2Bpl_ref(this);
-    call {:si_unique_call 43} {:cexpr "msg.sender"} boogie_si_record_sol2Bpl_ref(msgsender_MSG);
-    call {:si_unique_call 44} {:cexpr "msg.value"} boogie_si_record_sol2Bpl_int(msgvalue_MSG);
-    call {:si_unique_call 45} {:cexpr "_verisolLastArg"} boogie_si_record_sol2Bpl_bool(true);
+  anon9_Then:
+    assume {:partition} InstanceOwner_AssetTransfer[this] == msgsender_MSG;
     goto corral_source_split_37;
 
   corral_source_split_37:
     goto corral_source_split_38;
 
   corral_source_split_38:
-    goto anon5_Then, anon5_Else;
+    assume false;
+    goto anon6;
 
-  anon5_Then:
-    assume {:partition} StateEnum_SimpleMarketplace[this] != 1;
+  anon9_Else:
+    assume {:partition} InstanceOwner_AssetTransfer[this] != msgsender_MSG;
+    goto anon6;
+
+  anon6:
+    InstanceBuyer_AssetTransfer[this] := msgsender_MSG;
+    call {:si_unique_call 50} {:cexpr "InstanceBuyer"} boogie_si_record_sol2Bpl_ref(InstanceBuyer_AssetTransfer[this]);
     goto corral_source_split_40;
 
   corral_source_split_40:
+    InstanceInspector_AssetTransfer[this] := inspector_s310;
+    call {:si_unique_call 51} {:cexpr "InstanceInspector"} boogie_si_record_sol2Bpl_ref(InstanceInspector_AssetTransfer[this]);
     goto corral_source_split_41;
 
   corral_source_split_41:
+    InstanceAppraiser_AssetTransfer[this] := appraiser_s310;
+    call {:si_unique_call 52} {:cexpr "InstanceAppraiser"} boogie_si_record_sol2Bpl_ref(InstanceAppraiser_AssetTransfer[this]);
+    goto corral_source_split_42;
+
+  corral_source_split_42:
+    assume OfferPrice_AssetTransfer[this] >= 0;
+    assume offerPrice_s310 >= 0;
+    OfferPrice_AssetTransfer[this] := offerPrice_s310;
+    call {:si_unique_call 53} {:cexpr "OfferPrice"} boogie_si_record_sol2Bpl_int(OfferPrice_AssetTransfer[this]);
+    goto corral_source_split_43;
+
+  corral_source_split_43:
+    State_AssetTransfer[this] := 1;
+    return;
+}
+
+
+
+procedure {:public} AcceptOffer_AssetTransfer(this: Ref, msgsender_MSG: Ref, msgvalue_MSG: int);
+  modifies State_AssetTransfer;
+
+
+
+implementation {:ForceInline} AcceptOffer_AssetTransfer(this: Ref, msgsender_MSG: Ref, msgvalue_MSG: int)
+{
+
+  anon0:
+    call {:si_unique_call 54} {:cexpr "_verisolFirstArg"} boogie_si_record_sol2Bpl_bool(false);
+    call {:si_unique_call 55} {:cexpr "this"} boogie_si_record_sol2Bpl_ref(this);
+    call {:si_unique_call 56} {:cexpr "msg.sender"} boogie_si_record_sol2Bpl_ref(msgsender_MSG);
+    call {:si_unique_call 57} {:cexpr "msg.value"} boogie_si_record_sol2Bpl_int(msgvalue_MSG);
+    call {:si_unique_call 58} {:cexpr "_verisolLastArg"} boogie_si_record_sol2Bpl_bool(true);
+    goto corral_source_split_45;
+
+  corral_source_split_45:
+    goto corral_source_split_46;
+
+  corral_source_split_46:
+    goto anon5_Then, anon5_Else;
+
+  anon5_Then:
+    assume {:partition} State_AssetTransfer[this] != 1;
+    goto corral_source_split_48;
+
+  corral_source_split_48:
+    goto corral_source_split_49;
+
+  corral_source_split_49:
     assume false;
     goto anon2;
 
   anon5_Else:
-    assume {:partition} StateEnum_SimpleMarketplace[this] == 1;
+    assume {:partition} State_AssetTransfer[this] == 1;
     goto anon2;
 
   anon2:
     goto anon6_Then, anon6_Else;
 
   anon6_Then:
-    assume {:partition} msgsender_MSG != InstanceOwner_SimpleMarketplace[this];
-    goto corral_source_split_43;
+    assume {:partition} InstanceOwner_AssetTransfer[this] != msgsender_MSG;
+    goto corral_source_split_51;
 
-  corral_source_split_43:
-    goto corral_source_split_44;
+  corral_source_split_51:
+    goto corral_source_split_52;
 
-  corral_source_split_44:
+  corral_source_split_52:
     assume false;
     goto anon4;
 
   anon6_Else:
-    assume {:partition} msgsender_MSG == InstanceOwner_SimpleMarketplace[this];
+    assume {:partition} InstanceOwner_AssetTransfer[this] == msgsender_MSG;
     goto anon4;
 
   anon4:
-    StateEnum_SimpleMarketplace[this] := 2;
+    State_AssetTransfer[this] := 2;
+    return;
+}
+
+
+
+procedure {:public} Reject_AssetTransfer(this: Ref, msgsender_MSG: Ref, msgvalue_MSG: int);
+  modifies InstanceBuyer_AssetTransfer, State_AssetTransfer;
+
+
+
+implementation {:ForceInline} Reject_AssetTransfer(this: Ref, msgsender_MSG: Ref, msgvalue_MSG: int)
+{
+  var __var_3: Ref;
+
+  anon0:
+    call {:si_unique_call 59} {:cexpr "_verisolFirstArg"} boogie_si_record_sol2Bpl_bool(false);
+    call {:si_unique_call 60} {:cexpr "this"} boogie_si_record_sol2Bpl_ref(this);
+    call {:si_unique_call 61} {:cexpr "msg.sender"} boogie_si_record_sol2Bpl_ref(msgsender_MSG);
+    call {:si_unique_call 62} {:cexpr "msg.value"} boogie_si_record_sol2Bpl_int(msgvalue_MSG);
+    call {:si_unique_call 63} {:cexpr "_verisolLastArg"} boogie_si_record_sol2Bpl_bool(true);
+    goto corral_source_split_54;
+
+  corral_source_split_54:
+    goto corral_source_split_55;
+
+  corral_source_split_55:
+    goto anon5_Then, anon5_Else;
+
+  anon5_Then:
+    assume {:partition} State_AssetTransfer[this] != 1 && State_AssetTransfer[this] != 2 && State_AssetTransfer[this] != 3 && State_AssetTransfer[this] != 4 && State_AssetTransfer[this] != 5 && State_AssetTransfer[this] != 6;
+    goto corral_source_split_57;
+
+  corral_source_split_57:
+    goto corral_source_split_58;
+
+  corral_source_split_58:
+    assume false;
+    goto anon2;
+
+  anon5_Else:
+    assume {:partition} !(State_AssetTransfer[this] != 1 && State_AssetTransfer[this] != 2 && State_AssetTransfer[this] != 3 && State_AssetTransfer[this] != 4 && State_AssetTransfer[this] != 5 && State_AssetTransfer[this] != 6);
+    goto anon2;
+
+  anon2:
+    goto anon6_Then, anon6_Else;
+
+  anon6_Then:
+    assume {:partition} InstanceOwner_AssetTransfer[this] != msgsender_MSG;
+    goto corral_source_split_60;
+
+  corral_source_split_60:
+    goto corral_source_split_61;
+
+  corral_source_split_61:
+    assume false;
+    goto anon4;
+
+  anon6_Else:
+    assume {:partition} InstanceOwner_AssetTransfer[this] == msgsender_MSG;
+    goto anon4;
+
+  anon4:
+    __var_3 := null;
+    InstanceBuyer_AssetTransfer[this] := __var_3;
+    call {:si_unique_call 64} {:cexpr "InstanceBuyer"} boogie_si_record_sol2Bpl_ref(InstanceBuyer_AssetTransfer[this]);
+    goto corral_source_split_63;
+
+  corral_source_split_63:
+    State_AssetTransfer[this] := 0;
+    return;
+}
+
+
+
+procedure {:public} Accept_AssetTransfer(this: Ref, msgsender_MSG: Ref, msgvalue_MSG: int);
+  modifies State_AssetTransfer;
+
+
+
+implementation {:ForceInline} Accept_AssetTransfer(this: Ref, msgsender_MSG: Ref, msgvalue_MSG: int)
+{
+
+  anon0:
+    call {:si_unique_call 65} {:cexpr "_verisolFirstArg"} boogie_si_record_sol2Bpl_bool(false);
+    call {:si_unique_call 66} {:cexpr "this"} boogie_si_record_sol2Bpl_ref(this);
+    call {:si_unique_call 67} {:cexpr "msg.sender"} boogie_si_record_sol2Bpl_ref(msgsender_MSG);
+    call {:si_unique_call 68} {:cexpr "msg.value"} boogie_si_record_sol2Bpl_int(msgvalue_MSG);
+    call {:si_unique_call 69} {:cexpr "_verisolLastArg"} boogie_si_record_sol2Bpl_bool(true);
+    goto corral_source_split_65;
+
+  corral_source_split_65:
+    goto corral_source_split_66;
+
+  corral_source_split_66:
+    goto anon15_Then, anon15_Else;
+
+  anon15_Then:
+    assume {:partition} msgsender_MSG != InstanceBuyer_AssetTransfer[this] && msgsender_MSG != InstanceOwner_AssetTransfer[this];
+    goto corral_source_split_68;
+
+  corral_source_split_68:
+    goto corral_source_split_69;
+
+  corral_source_split_69:
+    assume false;
+    goto anon2;
+
+  anon15_Else:
+    assume {:partition} !(msgsender_MSG != InstanceBuyer_AssetTransfer[this] && msgsender_MSG != InstanceOwner_AssetTransfer[this]);
+    goto anon2;
+
+  anon2:
+    goto anon16_Then, anon16_Else;
+
+  anon16_Then:
+    assume {:partition} msgsender_MSG == InstanceOwner_AssetTransfer[this] && State_AssetTransfer[this] != 5 && State_AssetTransfer[this] != 6;
+    goto corral_source_split_71;
+
+  corral_source_split_71:
+    goto corral_source_split_72;
+
+  corral_source_split_72:
+    assume false;
+    goto anon4;
+
+  anon16_Else:
+    assume {:partition} !(msgsender_MSG == InstanceOwner_AssetTransfer[this] && State_AssetTransfer[this] != 5 && State_AssetTransfer[this] != 6);
+    goto anon4;
+
+  anon4:
+    goto anon17_Then, anon17_Else;
+
+  anon17_Then:
+    assume {:partition} msgsender_MSG == InstanceBuyer_AssetTransfer[this] && State_AssetTransfer[this] != 5 && State_AssetTransfer[this] != 7;
+    goto corral_source_split_74;
+
+  corral_source_split_74:
+    goto corral_source_split_75;
+
+  corral_source_split_75:
+    assume false;
+    goto anon6;
+
+  anon17_Else:
+    assume {:partition} !(msgsender_MSG == InstanceBuyer_AssetTransfer[this] && State_AssetTransfer[this] != 5 && State_AssetTransfer[this] != 7);
+    goto anon6;
+
+  anon6:
+    goto anon18_Then, anon18_Else;
+
+  anon18_Then:
+    assume {:partition} msgsender_MSG == InstanceBuyer_AssetTransfer[this];
+    goto corral_source_split_77;
+
+  corral_source_split_77:
+    goto corral_source_split_78;
+
+  corral_source_split_78:
+    goto anon19_Then, anon19_Else;
+
+  anon19_Then:
+    assume {:partition} State_AssetTransfer[this] == 5;
+    goto corral_source_split_80;
+
+  corral_source_split_80:
+    goto corral_source_split_81;
+
+  corral_source_split_81:
+    State_AssetTransfer[this] := 6;
+    return;
+
+  anon19_Else:
+    assume {:partition} State_AssetTransfer[this] != 5;
+    goto corral_source_split_83;
+
+  corral_source_split_83:
+    goto anon20_Then, anon20_Else;
+
+  anon20_Then:
+    assume {:partition} State_AssetTransfer[this] == 7;
+    goto corral_source_split_85;
+
+  corral_source_split_85:
+    goto corral_source_split_86;
+
+  corral_source_split_86:
+    State_AssetTransfer[this] := 8;
+    return;
+
+  anon20_Else:
+    assume {:partition} State_AssetTransfer[this] != 7;
+    return;
+
+  anon18_Else:
+    assume {:partition} msgsender_MSG != InstanceBuyer_AssetTransfer[this];
+    goto corral_source_split_88;
+
+  corral_source_split_88:
+    goto corral_source_split_89;
+
+  corral_source_split_89:
+    goto anon21_Then, anon21_Else;
+
+  anon21_Then:
+    assume {:partition} State_AssetTransfer[this] == 5;
+    goto corral_source_split_91;
+
+  corral_source_split_91:
+    goto corral_source_split_92;
+
+  corral_source_split_92:
+    State_AssetTransfer[this] := 7;
+    return;
+
+  anon21_Else:
+    assume {:partition} State_AssetTransfer[this] != 5;
+    goto corral_source_split_94;
+
+  corral_source_split_94:
+    goto anon22_Then, anon22_Else;
+
+  anon22_Then:
+    assume {:partition} State_AssetTransfer[this] == 6;
+    goto corral_source_split_96;
+
+  corral_source_split_96:
+    goto corral_source_split_97;
+
+  corral_source_split_97:
+    State_AssetTransfer[this] := 8;
+    return;
+
+  anon22_Else:
+    assume {:partition} State_AssetTransfer[this] != 6;
+    return;
+}
+
+
+
+procedure {:public} ModifyOffer_AssetTransfer(this: Ref, msgsender_MSG: Ref, msgvalue_MSG: int, offerPrice_s534: int);
+  modifies OfferPrice_AssetTransfer;
+
+
+
+implementation {:ForceInline} ModifyOffer_AssetTransfer(this: Ref, msgsender_MSG: Ref, msgvalue_MSG: int, offerPrice_s534: int)
+{
+
+  anon0:
+    call {:si_unique_call 70} {:cexpr "_verisolFirstArg"} boogie_si_record_sol2Bpl_bool(false);
+    call {:si_unique_call 71} {:cexpr "this"} boogie_si_record_sol2Bpl_ref(this);
+    call {:si_unique_call 72} {:cexpr "msg.sender"} boogie_si_record_sol2Bpl_ref(msgsender_MSG);
+    call {:si_unique_call 73} {:cexpr "msg.value"} boogie_si_record_sol2Bpl_int(msgvalue_MSG);
+    call {:si_unique_call 74} {:cexpr "offerPrice"} boogie_si_record_sol2Bpl_int(offerPrice_s534);
+    call {:si_unique_call 75} {:cexpr "_verisolLastArg"} boogie_si_record_sol2Bpl_bool(true);
+    goto corral_source_split_99;
+
+  corral_source_split_99:
+    goto corral_source_split_100;
+
+  corral_source_split_100:
+    goto anon5_Then, anon5_Else;
+
+  anon5_Then:
+    assume {:partition} State_AssetTransfer[this] != 1;
+    goto corral_source_split_102;
+
+  corral_source_split_102:
+    goto corral_source_split_103;
+
+  corral_source_split_103:
+    assume false;
+    goto anon2;
+
+  anon5_Else:
+    assume {:partition} State_AssetTransfer[this] == 1;
+    goto anon2;
+
+  anon2:
+    assume offerPrice_s534 >= 0;
+    goto anon6_Then, anon6_Else;
+
+  anon6_Then:
+    assume {:partition} InstanceBuyer_AssetTransfer[this] != msgsender_MSG || offerPrice_s534 == 0;
+    goto corral_source_split_105;
+
+  corral_source_split_105:
+    goto corral_source_split_106;
+
+  corral_source_split_106:
+    assume false;
+    goto anon4;
+
+  anon6_Else:
+    assume {:partition} !(InstanceBuyer_AssetTransfer[this] != msgsender_MSG || offerPrice_s534 == 0);
+    goto anon4;
+
+  anon4:
+    assume OfferPrice_AssetTransfer[this] >= 0;
+    assume offerPrice_s534 >= 0;
+    OfferPrice_AssetTransfer[this] := offerPrice_s534;
+    call {:si_unique_call 76} {:cexpr "OfferPrice"} boogie_si_record_sol2Bpl_int(OfferPrice_AssetTransfer[this]);
+    return;
+}
+
+
+
+procedure {:public} RescindOffer_AssetTransfer(this: Ref, msgsender_MSG: Ref, msgvalue_MSG: int);
+  modifies InstanceBuyer_AssetTransfer, OfferPrice_AssetTransfer, State_AssetTransfer;
+
+
+
+implementation {:ForceInline} RescindOffer_AssetTransfer(this: Ref, msgsender_MSG: Ref, msgvalue_MSG: int)
+{
+  var __var_4: Ref;
+
+  anon0:
+    call {:si_unique_call 77} {:cexpr "_verisolFirstArg"} boogie_si_record_sol2Bpl_bool(false);
+    call {:si_unique_call 78} {:cexpr "this"} boogie_si_record_sol2Bpl_ref(this);
+    call {:si_unique_call 79} {:cexpr "msg.sender"} boogie_si_record_sol2Bpl_ref(msgsender_MSG);
+    call {:si_unique_call 80} {:cexpr "msg.value"} boogie_si_record_sol2Bpl_int(msgvalue_MSG);
+    call {:si_unique_call 81} {:cexpr "_verisolLastArg"} boogie_si_record_sol2Bpl_bool(true);
+    goto corral_source_split_108;
+
+  corral_source_split_108:
+    goto corral_source_split_109;
+
+  corral_source_split_109:
+    goto anon5_Then, anon5_Else;
+
+  anon5_Then:
+    assume {:partition} State_AssetTransfer[this] != 1 && State_AssetTransfer[this] != 2 && State_AssetTransfer[this] != 3 && State_AssetTransfer[this] != 4 && State_AssetTransfer[this] != 5 && State_AssetTransfer[this] != 7;
+    goto corral_source_split_111;
+
+  corral_source_split_111:
+    goto corral_source_split_112;
+
+  corral_source_split_112:
+    assume false;
+    goto anon2;
+
+  anon5_Else:
+    assume {:partition} !(State_AssetTransfer[this] != 1 && State_AssetTransfer[this] != 2 && State_AssetTransfer[this] != 3 && State_AssetTransfer[this] != 4 && State_AssetTransfer[this] != 5 && State_AssetTransfer[this] != 7);
+    goto anon2;
+
+  anon2:
+    goto anon6_Then, anon6_Else;
+
+  anon6_Then:
+    assume {:partition} InstanceBuyer_AssetTransfer[this] != msgsender_MSG;
+    goto corral_source_split_114;
+
+  corral_source_split_114:
+    goto corral_source_split_115;
+
+  corral_source_split_115:
+    assume false;
+    goto anon4;
+
+  anon6_Else:
+    assume {:partition} InstanceBuyer_AssetTransfer[this] == msgsender_MSG;
+    goto anon4;
+
+  anon4:
+    __var_4 := null;
+    InstanceBuyer_AssetTransfer[this] := __var_4;
+    call {:si_unique_call 82} {:cexpr "InstanceBuyer"} boogie_si_record_sol2Bpl_ref(InstanceBuyer_AssetTransfer[this]);
+    goto corral_source_split_117;
+
+  corral_source_split_117:
+    assume OfferPrice_AssetTransfer[this] >= 0;
+    OfferPrice_AssetTransfer[this] := 0;
+    call {:si_unique_call 83} {:cexpr "OfferPrice"} boogie_si_record_sol2Bpl_int(OfferPrice_AssetTransfer[this]);
+    goto corral_source_split_118;
+
+  corral_source_split_118:
+    State_AssetTransfer[this] := 0;
+    return;
+}
+
+
+
+procedure {:public} MarkAppraised_AssetTransfer(this: Ref, msgsender_MSG: Ref, msgvalue_MSG: int);
+  modifies State_AssetTransfer;
+
+
+
+implementation {:ForceInline} MarkAppraised_AssetTransfer(this: Ref, msgsender_MSG: Ref, msgvalue_MSG: int)
+{
+
+  anon0:
+    call {:si_unique_call 84} {:cexpr "_verisolFirstArg"} boogie_si_record_sol2Bpl_bool(false);
+    call {:si_unique_call 85} {:cexpr "this"} boogie_si_record_sol2Bpl_ref(this);
+    call {:si_unique_call 86} {:cexpr "msg.sender"} boogie_si_record_sol2Bpl_ref(msgsender_MSG);
+    call {:si_unique_call 87} {:cexpr "msg.value"} boogie_si_record_sol2Bpl_int(msgvalue_MSG);
+    call {:si_unique_call 88} {:cexpr "_verisolLastArg"} boogie_si_record_sol2Bpl_bool(true);
+    goto corral_source_split_120;
+
+  corral_source_split_120:
+    goto corral_source_split_121;
+
+  corral_source_split_121:
+    goto anon7_Then, anon7_Else;
+
+  anon7_Then:
+    assume {:partition} InstanceAppraiser_AssetTransfer[this] != msgsender_MSG;
+    goto corral_source_split_123;
+
+  corral_source_split_123:
+    goto corral_source_split_124;
+
+  corral_source_split_124:
+    assume false;
+    goto anon2;
+
+  anon7_Else:
+    assume {:partition} InstanceAppraiser_AssetTransfer[this] == msgsender_MSG;
+    goto anon2;
+
+  anon2:
+    goto anon8_Then, anon8_Else;
+
+  anon8_Then:
+    assume {:partition} State_AssetTransfer[this] == 2;
+    goto corral_source_split_126;
+
+  corral_source_split_126:
+    goto corral_source_split_127;
+
+  corral_source_split_127:
+    State_AssetTransfer[this] := 4;
+    return;
+
+  anon8_Else:
+    assume {:partition} State_AssetTransfer[this] != 2;
+    goto corral_source_split_129;
+
+  corral_source_split_129:
+    goto anon9_Then, anon9_Else;
+
+  anon9_Then:
+    assume {:partition} State_AssetTransfer[this] == 3;
+    goto corral_source_split_131;
+
+  corral_source_split_131:
+    goto corral_source_split_132;
+
+  corral_source_split_132:
+    State_AssetTransfer[this] := 5;
+    return;
+
+  anon9_Else:
+    assume {:partition} State_AssetTransfer[this] != 3;
+    goto corral_source_split_134;
+
+  corral_source_split_134:
+    goto corral_source_split_135;
+
+  corral_source_split_135:
+    assume false;
+    return;
+}
+
+
+
+procedure {:public} MarkInspected_AssetTransfer(this: Ref, msgsender_MSG: Ref, msgvalue_MSG: int);
+  modifies State_AssetTransfer;
+
+
+
+implementation {:ForceInline} MarkInspected_AssetTransfer(this: Ref, msgsender_MSG: Ref, msgvalue_MSG: int)
+{
+
+  anon0:
+    call {:si_unique_call 89} {:cexpr "_verisolFirstArg"} boogie_si_record_sol2Bpl_bool(false);
+    call {:si_unique_call 90} {:cexpr "this"} boogie_si_record_sol2Bpl_ref(this);
+    call {:si_unique_call 91} {:cexpr "msg.sender"} boogie_si_record_sol2Bpl_ref(msgsender_MSG);
+    call {:si_unique_call 92} {:cexpr "msg.value"} boogie_si_record_sol2Bpl_int(msgvalue_MSG);
+    call {:si_unique_call 93} {:cexpr "_verisolLastArg"} boogie_si_record_sol2Bpl_bool(true);
+    goto corral_source_split_137;
+
+  corral_source_split_137:
+    goto corral_source_split_138;
+
+  corral_source_split_138:
+    goto anon7_Then, anon7_Else;
+
+  anon7_Then:
+    assume {:partition} InstanceInspector_AssetTransfer[this] != msgsender_MSG;
+    goto corral_source_split_140;
+
+  corral_source_split_140:
+    goto corral_source_split_141;
+
+  corral_source_split_141:
+    assume false;
+    goto anon2;
+
+  anon7_Else:
+    assume {:partition} InstanceInspector_AssetTransfer[this] == msgsender_MSG;
+    goto anon2;
+
+  anon2:
+    goto anon8_Then, anon8_Else;
+
+  anon8_Then:
+    assume {:partition} State_AssetTransfer[this] == 2;
+    goto corral_source_split_143;
+
+  corral_source_split_143:
+    goto corral_source_split_144;
+
+  corral_source_split_144:
+    State_AssetTransfer[this] := 3;
+    return;
+
+  anon8_Else:
+    assume {:partition} State_AssetTransfer[this] != 2;
+    goto corral_source_split_146;
+
+  corral_source_split_146:
+    goto anon9_Then, anon9_Else;
+
+  anon9_Then:
+    assume {:partition} State_AssetTransfer[this] == 4;
+    goto corral_source_split_148;
+
+  corral_source_split_148:
+    goto corral_source_split_149;
+
+  corral_source_split_149:
+    State_AssetTransfer[this] := 5;
+    return;
+
+  anon9_Else:
+    assume {:partition} State_AssetTransfer[this] != 4;
+    goto corral_source_split_151;
+
+  corral_source_split_151:
+    goto corral_source_split_152;
+
+  corral_source_split_152:
+    assume false;
     return;
 }
 
@@ -449,115 +1054,221 @@ procedure send(from: Ref, to: Ref, amount: int) returns (success: bool);
 
 
 
-const {:existential true} HoudiniB1_SimpleMarketplace: bool;
+const {:existential true} HoudiniB1_AssetTransfer: bool;
 
-const {:existential true} HoudiniB2_SimpleMarketplace: bool;
+const {:existential true} HoudiniB2_AssetTransfer: bool;
 
-const {:existential true} HoudiniB3_SimpleMarketplace: bool;
+const {:existential true} HoudiniB3_AssetTransfer: bool;
 
-const {:existential true} HoudiniB4_SimpleMarketplace: bool;
+const {:existential true} HoudiniB4_AssetTransfer: bool;
 
-const {:existential true} HoudiniB5_SimpleMarketplace: bool;
+const {:existential true} HoudiniB5_AssetTransfer: bool;
 
-const {:existential true} HoudiniB6_SimpleMarketplace: bool;
+const {:existential true} HoudiniB6_AssetTransfer: bool;
 
-procedure BoogieEntry_SimpleMarketplace();
+const {:existential true} HoudiniB7_AssetTransfer: bool;
+
+const {:existential true} HoudiniB8_AssetTransfer: bool;
+
+const {:existential true} HoudiniB9_AssetTransfer: bool;
+
+const {:existential true} HoudiniB10_AssetTransfer: bool;
+
+const {:existential true} HoudiniB11_AssetTransfer: bool;
+
+const {:existential true} HoudiniB12_AssetTransfer: bool;
+
+const {:existential true} HoudiniB13_AssetTransfer: bool;
+
+const {:existential true} HoudiniB14_AssetTransfer: bool;
+
+const {:existential true} HoudiniB15_AssetTransfer: bool;
+
+const {:existential true} HoudiniB16_AssetTransfer: bool;
+
+const {:existential true} HoudiniB17_AssetTransfer: bool;
+
+const {:existential true} HoudiniB18_AssetTransfer: bool;
+
+const {:existential true} HoudiniB19_AssetTransfer: bool;
+
+const {:existential true} HoudiniB20_AssetTransfer: bool;
+
+procedure BoogieEntry_AssetTransfer();
 
 
 
-procedure CorralChoice_SimpleMarketplace(this: Ref);
-  modifies now, Alloc, InstanceBuyer_SimpleMarketplace, OfferPrice_SimpleMarketplace, StateEnum_SimpleMarketplace;
+procedure CorralChoice_AssetTransfer(this: Ref);
+  modifies now, Alloc, State_AssetTransfer, Description_AssetTransfer, AskingPrice_AssetTransfer, InstanceBuyer_AssetTransfer, InstanceInspector_AssetTransfer, InstanceAppraiser_AssetTransfer, OfferPrice_AssetTransfer;
 
 
 
-implementation CorralChoice_SimpleMarketplace(this: Ref)
+implementation CorralChoice_AssetTransfer(this: Ref)
 {
   var msgsender_MSG: Ref;
   var msgvalue_MSG: int;
   var choice: int;
-  var offerPrice_s60: int;
-  var description_s107: int;
-  var price_s107: int;
-  var sender_s107: Ref;
-  var offerPrice_s153: int;
+  var offerPrice_s135: int;
+  var inspector_s135: Ref;
+  var appraiser_s135: Ref;
+  var description_s135: int;
+  var price_s135: int;
+  var description_s188: int;
+  var price_s188: int;
+  var description_s240: int;
+  var price_s240: int;
+  var inspector_s310: Ref;
+  var appraiser_s310: Ref;
+  var offerPrice_s310: int;
+  var offerPrice_s534: int;
   var tmpNow: int;
 
   anon0:
     havoc msgsender_MSG;
     havoc msgvalue_MSG;
     havoc choice;
-    havoc offerPrice_s60;
-    havoc description_s107;
-    havoc price_s107;
-    havoc sender_s107;
-    havoc offerPrice_s153;
+    havoc offerPrice_s135;
+    havoc inspector_s135;
+    havoc appraiser_s135;
+    havoc description_s135;
+    havoc price_s135;
+    havoc description_s188;
+    havoc price_s188;
+    havoc description_s240;
+    havoc price_s240;
+    havoc inspector_s310;
+    havoc appraiser_s310;
+    havoc offerPrice_s310;
+    havoc offerPrice_s534;
     havoc tmpNow;
     tmpNow := now;
     havoc now;
     assume now > tmpNow;
     assume msgsender_MSG != null;
-    assume DType[msgsender_MSG] != SimpleMarketplace;
+    assume DType[msgsender_MSG] != AssetTransfer;
     Alloc[msgsender_MSG] := true;
-    goto anon5_Then, anon5_Else;
+    goto anon12_Then, anon12_Else;
 
-  anon5_Then:
+  anon12_Then:
+    assume {:partition} choice == 11;
+    call {:si_unique_call 94} prueba_AssetTransfer(this, msgsender_MSG, msgvalue_MSG, offerPrice_s135, inspector_s135, appraiser_s135, description_s135, price_s135);
+    return;
+
+  anon12_Else:
+    assume {:partition} choice != 11;
+    goto anon13_Then, anon13_Else;
+
+  anon13_Then:
+    assume {:partition} choice == 10;
+    call {:si_unique_call 95} Terminate_AssetTransfer(this, msgsender_MSG, msgvalue_MSG);
+    return;
+
+  anon13_Else:
+    assume {:partition} choice != 10;
+    goto anon14_Then, anon14_Else;
+
+  anon14_Then:
+    assume {:partition} choice == 9;
+    call {:si_unique_call 96} Modify_AssetTransfer(this, msgsender_MSG, msgvalue_MSG, description_s240, price_s240);
+    return;
+
+  anon14_Else:
+    assume {:partition} choice != 9;
+    goto anon15_Then, anon15_Else;
+
+  anon15_Then:
+    assume {:partition} choice == 8;
+    call {:si_unique_call 97} MakeOffer_AssetTransfer(this, msgsender_MSG, msgvalue_MSG, inspector_s310, appraiser_s310, offerPrice_s310);
+    return;
+
+  anon15_Else:
+    assume {:partition} choice != 8;
+    goto anon16_Then, anon16_Else;
+
+  anon16_Then:
+    assume {:partition} choice == 7;
+    call {:si_unique_call 98} AcceptOffer_AssetTransfer(this, msgsender_MSG, msgvalue_MSG);
+    return;
+
+  anon16_Else:
+    assume {:partition} choice != 7;
+    goto anon17_Then, anon17_Else;
+
+  anon17_Then:
+    assume {:partition} choice == 6;
+    call {:si_unique_call 99} Reject_AssetTransfer(this, msgsender_MSG, msgvalue_MSG);
+    return;
+
+  anon17_Else:
+    assume {:partition} choice != 6;
+    goto anon18_Then, anon18_Else;
+
+  anon18_Then:
+    assume {:partition} choice == 5;
+    call {:si_unique_call 100} Accept_AssetTransfer(this, msgsender_MSG, msgvalue_MSG);
+    return;
+
+  anon18_Else:
+    assume {:partition} choice != 5;
+    goto anon19_Then, anon19_Else;
+
+  anon19_Then:
     assume {:partition} choice == 4;
-    call {:si_unique_call 46} prueba_SimpleMarketplace(this, msgsender_MSG, msgvalue_MSG, offerPrice_s60);
+    call {:si_unique_call 101} ModifyOffer_AssetTransfer(this, msgsender_MSG, msgvalue_MSG, offerPrice_s534);
     return;
 
-  anon5_Else:
+  anon19_Else:
     assume {:partition} choice != 4;
-    goto anon6_Then, anon6_Else;
+    goto anon20_Then, anon20_Else;
 
-  anon6_Then:
+  anon20_Then:
     assume {:partition} choice == 3;
-    call {:si_unique_call 47} MakeOffer_SimpleMarketplace(this, msgsender_MSG, msgvalue_MSG, offerPrice_s153);
+    call {:si_unique_call 102} RescindOffer_AssetTransfer(this, msgsender_MSG, msgvalue_MSG);
     return;
 
-  anon6_Else:
+  anon20_Else:
     assume {:partition} choice != 3;
-    goto anon7_Then, anon7_Else;
+    goto anon21_Then, anon21_Else;
 
-  anon7_Then:
+  anon21_Then:
     assume {:partition} choice == 2;
-    call {:si_unique_call 48} Reject_SimpleMarketplace(this, msgsender_MSG, msgvalue_MSG);
+    call {:si_unique_call 103} MarkAppraised_AssetTransfer(this, msgsender_MSG, msgvalue_MSG);
     return;
 
-  anon7_Else:
+  anon21_Else:
     assume {:partition} choice != 2;
-    goto anon8_Then, anon8_Else;
+    goto anon22_Then, anon22_Else;
 
-  anon8_Then:
+  anon22_Then:
     assume {:partition} choice == 1;
-    call {:si_unique_call 49} AcceptOffer_SimpleMarketplace(this, msgsender_MSG, msgvalue_MSG);
+    call {:si_unique_call 104} MarkInspected_AssetTransfer(this, msgsender_MSG, msgvalue_MSG);
     return;
 
-  anon8_Else:
+  anon22_Else:
     assume {:partition} choice != 1;
     return;
 }
 
 
 
-procedure CorralEntry_SimpleMarketplace();
-  modifies Alloc, Balance, InstanceOwner_SimpleMarketplace, Description_SimpleMarketplace, AskingPrice_SimpleMarketplace, result_SimpleMarketplace, InstanceBuyer_SimpleMarketplace, OfferPrice_SimpleMarketplace, StateEnum_SimpleMarketplace, now;
+procedure CorralEntry_AssetTransfer();
+  modifies Alloc, Balance, InstanceOwner_AssetTransfer, Description_AssetTransfer, AskingPrice_AssetTransfer, InstanceBuyer_AssetTransfer, OfferPrice_AssetTransfer, InstanceInspector_AssetTransfer, InstanceAppraiser_AssetTransfer, State_AssetTransfer, now;
 
 
 
-implementation CorralEntry_SimpleMarketplace()
+implementation CorralEntry_AssetTransfer()
 {
   var this: Ref;
   var msgsender_MSG: Ref;
   var msgvalue_MSG: int;
-  var description_s107: int;
-  var price_s107: int;
-  var sender_s107: Ref;
+  var description_s188: int;
+  var price_s188: int;
 
   anon0:
-    call {:si_unique_call 50} this := FreshRefGenerator();
+    call {:si_unique_call 105} this := FreshRefGenerator();
     assume now >= 0;
-    assume DType[this] == SimpleMarketplace;
-    call {:si_unique_call 51} SimpleMarketplace_SimpleMarketplace(this, msgsender_MSG, msgvalue_MSG, description_s107, price_s107, sender_s107);
+    assume DType[this] == AssetTransfer;
+    call {:si_unique_call 106} AssetTransfer_AssetTransfer(this, msgsender_MSG, msgvalue_MSG, description_s188, price_s188);
     goto anon2_LoopHead;
 
   anon2_LoopHead:
@@ -565,7 +1276,7 @@ implementation CorralEntry_SimpleMarketplace()
 
   anon2_LoopBody:
     assume {:partition} true;
-    call {:si_unique_call 52} CorralChoice_SimpleMarketplace(this);
+    call {:si_unique_call 107} CorralChoice_AssetTransfer(this);
     goto anon2_LoopHead;
 
   anon2_LoopDone:
