2/new_folder3/corral_out.bpl
@@ -4,7 +4,7 @@ type ContractName;
 
 const unique null: Ref;
 
-const unique SimpleMarketplace: ContractName;
+const unique RoomThermostat: ContractName;
 
 function ConstantToRef(x: int) : Ref;
 
@@ -31,10 +31,6 @@ var DType: [Ref]ContractName;
 var Alloc: [Ref]bool;
 
 var balance_ADDR: [Ref]int;
-
-var M_int_int: [Ref][int]int;
-
-var M_int_Ref: [Ref][int]Ref;
 
 var Length: [Ref]int;
 
@@ -90,11 +86,11 @@ axiom (forall __i__0_0: Ref, __i__0_1: Ref :: { abiEncodePacked1R(__i__0_0), abi
 
 axiom (forall __i__0_0: Ref, __i__0_1: Ref, __i__1_0: int, __i__1_1: int :: { abiEncodePacked2R(__i__0_0, __i__1_0), abiEncodePacked2R(__i__0_1, __i__1_1) } (__i__0_0 == __i__0_1 && __i__1_0 == __i__1_1) || abiEncodePacked2R(__i__0_0, __i__1_0) != abiEncodePacked2R(__i__0_1, __i__1_1));
 
-procedure {:public} prueba_SimpleMarketplace(this: Ref, msgsender_MSG: Ref, msgvalue_MSG: int, offerPrice_s31: int);
+procedure {:public} prueba_RoomThermostat(this: Ref, msgsender_MSG: Ref, msgvalue_MSG: int, targetTemperature_s32: int, mode_s32: int);
 
 
 
-implementation {:ForceInline} prueba_SimpleMarketplace(this: Ref, msgsender_MSG: Ref, msgvalue_MSG: int, offerPrice_s31: int)
+implementation {:ForceInline} prueba_RoomThermostat(this: Ref, msgsender_MSG: Ref, msgvalue_MSG: int, targetTemperature_s32: int, mode_s32: int)
 {
 
   anon0:
@@ -102,7 +98,7 @@ implementation {:ForceInline} prueba_SimpleMarketplace(this: Ref, msgsender_MSG:
     call {:si_unique_call 1} {:cexpr "this"} boogie_si_record_sol2Bpl_ref(this);
     call {:si_unique_call 2} {:cexpr "msg.sender"} boogie_si_record_sol2Bpl_ref(msgsender_MSG);
     call {:si_unique_call 3} {:cexpr "msg.value"} boogie_si_record_sol2Bpl_int(msgvalue_MSG);
-    call {:si_unique_call 4} {:cexpr "offerPrice"} boogie_si_record_sol2Bpl_int(offerPrice_s31);
+    call {:si_unique_call 4} {:cexpr "targetTemperature"} boogie_si_record_sol2Bpl_int(targetTemperature_s32);
     call {:si_unique_call 5} {:cexpr "_verisolLastArg"} boogie_si_record_sol2Bpl_bool(true);
     goto corral_source_split_1;
 
@@ -110,7 +106,7 @@ implementation {:ForceInline} prueba_SimpleMarketplace(this: Ref, msgsender_MSG:
     goto corral_source_split_2;
 
   corral_source_split_2:
-    assume !(StateEnum_SimpleMarketplace[this] == 0) && StateEnum_SimpleMarketplace[this] == 1 && StateEnum_SimpleMarketplace[this] == 1;
+    assume !(State_RoomThermostat[this] == 0) && State_RoomThermostat[this] == 1 && State_RoomThermostat[this] == 1;
     goto corral_source_split_3;
 
   corral_source_split_3:
@@ -120,124 +116,110 @@ implementation {:ForceInline} prueba_SimpleMarketplace(this: Ref, msgsender_MSG:
 
 
 
-var InstanceOwner_SimpleMarketplace: [Ref]Ref;
+var State_RoomThermostat: [Ref]int;
 
-var Description_SimpleMarketplace: [Ref]int;
+var Installer_RoomThermostat: [Ref]Ref;
 
-var AskingPrice_SimpleMarketplace: [Ref]int;
+var User_RoomThermostat: [Ref]Ref;
 
-var StateEnum_SimpleMarketplace: [Ref]int;
+var TargetTemperature_RoomThermostat: [Ref]int;
 
-var result_SimpleMarketplace: [Ref]Ref;
+var Mode_RoomThermostat: [Ref]int;
 
-var InstanceBuyer_SimpleMarketplace: [Ref]Ref;
-
-var OfferPrice_SimpleMarketplace: [Ref]int;
-
-procedure SimpleMarketplace_SimpleMarketplace_NoBaseCtor(this: Ref, msgsender_MSG: Ref, msgvalue_MSG: int, description_s78: int, price_s78: int, sender_s78: Ref);
-  modifies Balance, InstanceOwner_SimpleMarketplace, Description_SimpleMarketplace, AskingPrice_SimpleMarketplace, Alloc, result_SimpleMarketplace, InstanceBuyer_SimpleMarketplace, OfferPrice_SimpleMarketplace, StateEnum_SimpleMarketplace;
+procedure RoomThermostat_RoomThermostat_NoBaseCtor(this: Ref, msgsender_MSG: Ref, msgvalue_MSG: int, thermostatInstaller_s75: Ref, thermostatUser_s75: Ref);
+  modifies Balance, Installer_RoomThermostat, User_RoomThermostat, TargetTemperature_RoomThermostat, State_RoomThermostat;
 
 
 
-implementation {:ForceInline} SimpleMarketplace_SimpleMarketplace_NoBaseCtor(this: Ref, msgsender_MSG: Ref, msgvalue_MSG: int, description_s78: int, price_s78: int, sender_s78: Ref)
+implementation {:ForceInline} RoomThermostat_RoomThermostat_NoBaseCtor(this: Ref, msgsender_MSG: Ref, msgvalue_MSG: int, thermostatInstaller_s75: Ref, thermostatUser_s75: Ref)
 {
-  var __var_1: Ref;
 
   anon0:
     assume msgsender_MSG != null;
     Balance[this] := 0;
-    InstanceOwner_SimpleMarketplace[this] := null;
-    Description_SimpleMarketplace[this] := -2097454804;
-    AskingPrice_SimpleMarketplace[this] := 0;
-    call {:si_unique_call 6} __var_1 := FreshRefGenerator();
-    result_SimpleMarketplace[this] := __var_1;
-    assume Length[result_SimpleMarketplace[this]] == 0;
-    InstanceBuyer_SimpleMarketplace[this] := null;
-    OfferPrice_SimpleMarketplace[this] := 0;
-    call {:si_unique_call 7} {:cexpr "_verisolFirstArg"} boogie_si_record_sol2Bpl_bool(false);
-    call {:si_unique_call 8} {:cexpr "this"} boogie_si_record_sol2Bpl_ref(this);
-    call {:si_unique_call 9} {:cexpr "msg.sender"} boogie_si_record_sol2Bpl_ref(msgsender_MSG);
-    call {:si_unique_call 10} {:cexpr "msg.value"} boogie_si_record_sol2Bpl_int(msgvalue_MSG);
-    call {:si_unique_call 11} {:cexpr "description"} boogie_si_record_sol2Bpl_int(description_s78);
-    call {:si_unique_call 12} {:cexpr "price"} boogie_si_record_sol2Bpl_int(price_s78);
-    call {:si_unique_call 13} {:cexpr "sender"} boogie_si_record_sol2Bpl_ref(sender_s78);
-    call {:si_unique_call 14} {:cexpr "_verisolLastArg"} boogie_si_record_sol2Bpl_bool(true);
+    Installer_RoomThermostat[this] := null;
+    User_RoomThermostat[this] := null;
+    TargetTemperature_RoomThermostat[this] := 0;
+    call {:si_unique_call 6} {:cexpr "_verisolFirstArg"} boogie_si_record_sol2Bpl_bool(false);
+    call {:si_unique_call 7} {:cexpr "this"} boogie_si_record_sol2Bpl_ref(this);
+    call {:si_unique_call 8} {:cexpr "msg.sender"} boogie_si_record_sol2Bpl_ref(msgsender_MSG);
+    call {:si_unique_call 9} {:cexpr "msg.value"} boogie_si_record_sol2Bpl_int(msgvalue_MSG);
+    call {:si_unique_call 10} {:cexpr "thermostatInstaller"} boogie_si_record_sol2Bpl_ref(thermostatInstaller_s75);
+    call {:si_unique_call 11} {:cexpr "thermostatUser"} boogie_si_record_sol2Bpl_ref(thermostatUser_s75);
+    call {:si_unique_call 12} {:cexpr "_verisolLastArg"} boogie_si_record_sol2Bpl_bool(true);
     goto corral_source_split_5;
 
   corral_source_split_5:
     goto corral_source_split_6;
 
   corral_source_split_6:
-    InstanceOwner_SimpleMarketplace[this] := sender_s78;
-    call {:si_unique_call 15} {:cexpr "InstanceOwner"} boogie_si_record_sol2Bpl_ref(InstanceOwner_SimpleMarketplace[this]);
+    Installer_RoomThermostat[this] := thermostatInstaller_s75;
+    call {:si_unique_call 13} {:cexpr "Installer"} boogie_si_record_sol2Bpl_ref(Installer_RoomThermostat[this]);
     goto corral_source_split_7;
 
   corral_source_split_7:
-    AskingPrice_SimpleMarketplace[this] := price_s78;
-    call {:si_unique_call 16} {:cexpr "AskingPrice"} boogie_si_record_sol2Bpl_int(AskingPrice_SimpleMarketplace[this]);
+    User_RoomThermostat[this] := thermostatUser_s75;
+    call {:si_unique_call 14} {:cexpr "User"} boogie_si_record_sol2Bpl_ref(User_RoomThermostat[this]);
     goto corral_source_split_8;
 
   corral_source_split_8:
-    Description_SimpleMarketplace[this] := description_s78;
-    call {:si_unique_call 17} {:cexpr "Description"} boogie_si_record_sol2Bpl_int(Description_SimpleMarketplace[this]);
+    TargetTemperature_RoomThermostat[this] := 70;
+    call {:si_unique_call 15} {:cexpr "TargetTemperature"} boogie_si_record_sol2Bpl_int(TargetTemperature_RoomThermostat[this]);
     goto corral_source_split_9;
 
   corral_source_split_9:
-    StateEnum_SimpleMarketplace[this] := 0;
+    State_RoomThermostat[this] := 0;
     return;
 }
 
 
 
-procedure {:constructor} {:public} SimpleMarketplace_SimpleMarketplace(this: Ref, msgsender_MSG: Ref, msgvalue_MSG: int, description_s78: int, price_s78: int, sender_s78: Ref);
-  modifies Balance, InstanceOwner_SimpleMarketplace, Description_SimpleMarketplace, AskingPrice_SimpleMarketplace, Alloc, result_SimpleMarketplace, InstanceBuyer_SimpleMarketplace, OfferPrice_SimpleMarketplace, StateEnum_SimpleMarketplace;
+procedure {:constructor} {:public} RoomThermostat_RoomThermostat(this: Ref, msgsender_MSG: Ref, msgvalue_MSG: int, thermostatInstaller_s75: Ref, thermostatUser_s75: Ref);
+  modifies Balance, Installer_RoomThermostat, User_RoomThermostat, TargetTemperature_RoomThermostat, State_RoomThermostat;
 
 
 
-implementation {:ForceInline} SimpleMarketplace_SimpleMarketplace(this: Ref, msgsender_MSG: Ref, msgvalue_MSG: int, description_s78: int, price_s78: int, sender_s78: Ref)
+implementation {:ForceInline} RoomThermostat_RoomThermostat(this: Ref, msgsender_MSG: Ref, msgvalue_MSG: int, thermostatInstaller_s75: Ref, thermostatUser_s75: Ref)
 {
-  var __var_1: Ref;
 
   anon0:
-    call {:si_unique_call 18} {:cexpr "_verisolFirstArg"} boogie_si_record_sol2Bpl_bool(false);
-    call {:si_unique_call 19} {:cexpr "this"} boogie_si_record_sol2Bpl_ref(this);
-    call {:si_unique_call 20} {:cexpr "msg.sender"} boogie_si_record_sol2Bpl_ref(msgsender_MSG);
-    call {:si_unique_call 21} {:cexpr "msg.value"} boogie_si_record_sol2Bpl_int(msgvalue_MSG);
-    call {:si_unique_call 22} {:cexpr "description"} boogie_si_record_sol2Bpl_int(description_s78);
-    call {:si_unique_call 23} {:cexpr "price"} boogie_si_record_sol2Bpl_int(price_s78);
-    call {:si_unique_call 24} {:cexpr "sender"} boogie_si_record_sol2Bpl_ref(sender_s78);
-    call {:si_unique_call 25} {:cexpr "_verisolLastArg"} boogie_si_record_sol2Bpl_bool(true);
-    call {:si_unique_call 26} SimpleMarketplace_SimpleMarketplace_NoBaseCtor(this, msgsender_MSG, msgvalue_MSG, description_s78, price_s78, sender_s78);
+    call {:si_unique_call 16} {:cexpr "_verisolFirstArg"} boogie_si_record_sol2Bpl_bool(false);
+    call {:si_unique_call 17} {:cexpr "this"} boogie_si_record_sol2Bpl_ref(this);
+    call {:si_unique_call 18} {:cexpr "msg.sender"} boogie_si_record_sol2Bpl_ref(msgsender_MSG);
+    call {:si_unique_call 19} {:cexpr "msg.value"} boogie_si_record_sol2Bpl_int(msgvalue_MSG);
+    call {:si_unique_call 20} {:cexpr "thermostatInstaller"} boogie_si_record_sol2Bpl_ref(thermostatInstaller_s75);
+    call {:si_unique_call 21} {:cexpr "thermostatUser"} boogie_si_record_sol2Bpl_ref(thermostatUser_s75);
+    call {:si_unique_call 22} {:cexpr "_verisolLastArg"} boogie_si_record_sol2Bpl_bool(true);
+    call {:si_unique_call 23} RoomThermostat_RoomThermostat_NoBaseCtor(this, msgsender_MSG, msgvalue_MSG, thermostatInstaller_s75, thermostatUser_s75);
     return;
 }
 
 
 
-procedure {:public} MakeOffer_SimpleMarketplace(this: Ref, msgsender_MSG: Ref, msgvalue_MSG: int, offerPrice_s124: int);
-  modifies InstanceBuyer_SimpleMarketplace, OfferPrice_SimpleMarketplace, StateEnum_SimpleMarketplace;
+procedure {:public} StartThermostat_RoomThermostat(this: Ref, msgsender_MSG: Ref, msgvalue_MSG: int);
+  modifies State_RoomThermostat;
 
 
 
-implementation {:ForceInline} MakeOffer_SimpleMarketplace(this: Ref, msgsender_MSG: Ref, msgvalue_MSG: int, offerPrice_s124: int)
+implementation {:ForceInline} StartThermostat_RoomThermostat(this: Ref, msgsender_MSG: Ref, msgvalue_MSG: int)
 {
 
   anon0:
-    call {:si_unique_call 27} {:cexpr "_verisolFirstArg"} boogie_si_record_sol2Bpl_bool(false);
-    call {:si_unique_call 28} {:cexpr "this"} boogie_si_record_sol2Bpl_ref(this);
-    call {:si_unique_call 29} {:cexpr "msg.sender"} boogie_si_record_sol2Bpl_ref(msgsender_MSG);
-    call {:si_unique_call 30} {:cexpr "msg.value"} boogie_si_record_sol2Bpl_int(msgvalue_MSG);
-    call {:si_unique_call 31} {:cexpr "offerPrice"} boogie_si_record_sol2Bpl_int(offerPrice_s124);
-    call {:si_unique_call 32} {:cexpr "_verisolLastArg"} boogie_si_record_sol2Bpl_bool(true);
+    call {:si_unique_call 24} {:cexpr "_verisolFirstArg"} boogie_si_record_sol2Bpl_bool(false);
+    call {:si_unique_call 25} {:cexpr "this"} boogie_si_record_sol2Bpl_ref(this);
+    call {:si_unique_call 26} {:cexpr "msg.sender"} boogie_si_record_sol2Bpl_ref(msgsender_MSG);
+    call {:si_unique_call 27} {:cexpr "msg.value"} boogie_si_record_sol2Bpl_int(msgvalue_MSG);
+    call {:si_unique_call 28} {:cexpr "_verisolLastArg"} boogie_si_record_sol2Bpl_bool(true);
     goto corral_source_split_11;
 
   corral_source_split_11:
     goto corral_source_split_12;
 
   corral_source_split_12:
-    goto anon7_Then, anon7_Else;
+    goto anon3_Then, anon3_Else;
 
-  anon7_Then:
-    assume {:partition} offerPrice_s124 == 0;
+  anon3_Then:
+    assume {:partition} Installer_RoomThermostat[this] != msgsender_MSG || State_RoomThermostat[this] != 0;
     goto corral_source_split_14;
 
   corral_source_split_14:
@@ -247,33 +229,42 @@ implementation {:ForceInline} MakeOffer_SimpleMarketplace(this: Ref, msgsender_M
     assume false;
     goto anon2;
 
-  anon7_Else:
-    assume {:partition} offerPrice_s124 != 0;
+  anon3_Else:
+    assume {:partition} !(Installer_RoomThermostat[this] != msgsender_MSG || State_RoomThermostat[this] != 0);
     goto anon2;
 
   anon2:
-    goto anon8_Then, anon8_Else;
+    State_RoomThermostat[this] := 1;
+    return;
+}
 
-  anon8_Then:
-    assume {:partition} StateEnum_SimpleMarketplace[this] != 0;
+
+
+procedure {:public} SetTargetTemperature_RoomThermostat(this: Ref, msgsender_MSG: Ref, msgvalue_MSG: int, targetTemperature_s122: int);
+  modifies TargetTemperature_RoomThermostat;
+
+
+
+implementation {:ForceInline} SetTargetTemperature_RoomThermostat(this: Ref, msgsender_MSG: Ref, msgvalue_MSG: int, targetTemperature_s122: int)
+{
+
+  anon0:
+    call {:si_unique_call 29} {:cexpr "_verisolFirstArg"} boogie_si_record_sol2Bpl_bool(false);
+    call {:si_unique_call 30} {:cexpr "this"} boogie_si_record_sol2Bpl_ref(this);
+    call {:si_unique_call 31} {:cexpr "msg.sender"} boogie_si_record_sol2Bpl_ref(msgsender_MSG);
+    call {:si_unique_call 32} {:cexpr "msg.value"} boogie_si_record_sol2Bpl_int(msgvalue_MSG);
+    call {:si_unique_call 33} {:cexpr "targetTemperature"} boogie_si_record_sol2Bpl_int(targetTemperature_s122);
+    call {:si_unique_call 34} {:cexpr "_verisolLastArg"} boogie_si_record_sol2Bpl_bool(true);
     goto corral_source_split_17;
 
   corral_source_split_17:
     goto corral_source_split_18;
 
   corral_source_split_18:
-    assume false;
-    goto anon4;
+    goto anon3_Then, anon3_Else;
 
-  anon8_Else:
-    assume {:partition} StateEnum_SimpleMarketplace[this] == 0;
-    goto anon4;
-
-  anon4:
-    goto anon9_Then, anon9_Else;
-
-  anon9_Then:
-    assume {:partition} InstanceOwner_SimpleMarketplace[this] == msgsender_MSG;
+  anon3_Then:
+    assume {:partition} User_RoomThermostat[this] != msgsender_MSG || State_RoomThermostat[this] != 1;
     goto corral_source_split_20;
 
   corral_source_split_20:
@@ -281,148 +272,59 @@ implementation {:ForceInline} MakeOffer_SimpleMarketplace(this: Ref, msgsender_M
 
   corral_source_split_21:
     assume false;
-    goto anon6;
+    goto anon2;
 
-  anon9_Else:
-    assume {:partition} InstanceOwner_SimpleMarketplace[this] != msgsender_MSG;
-    goto anon6;
+  anon3_Else:
+    assume {:partition} !(User_RoomThermostat[this] != msgsender_MSG || State_RoomThermostat[this] != 1);
+    goto anon2;
 
-  anon6:
-    InstanceBuyer_SimpleMarketplace[this] := msgsender_MSG;
-    call {:si_unique_call 33} {:cexpr "InstanceBuyer"} boogie_si_record_sol2Bpl_ref(InstanceBuyer_SimpleMarketplace[this]);
-    goto corral_source_split_23;
-
-  corral_source_split_23:
-    OfferPrice_SimpleMarketplace[this] := offerPrice_s124;
-    call {:si_unique_call 34} {:cexpr "OfferPrice"} boogie_si_record_sol2Bpl_int(OfferPrice_SimpleMarketplace[this]);
-    goto corral_source_split_24;
-
-  corral_source_split_24:
-    StateEnum_SimpleMarketplace[this] := 1;
+  anon2:
+    TargetTemperature_RoomThermostat[this] := targetTemperature_s122;
+    call {:si_unique_call 35} {:cexpr "TargetTemperature"} boogie_si_record_sol2Bpl_int(TargetTemperature_RoomThermostat[this]);
     return;
 }
 
 
 
-procedure {:public} Reject_SimpleMarketplace(this: Ref, msgsender_MSG: Ref, msgvalue_MSG: int);
-  modifies StateEnum_SimpleMarketplace;
+procedure {:public} SetMode_RoomThermostat(this: Ref, msgsender_MSG: Ref, msgvalue_MSG: int, mode_s146: int);
+  modifies Mode_RoomThermostat;
 
 
 
-implementation {:ForceInline} Reject_SimpleMarketplace(this: Ref, msgsender_MSG: Ref, msgvalue_MSG: int)
+implementation {:ForceInline} SetMode_RoomThermostat(this: Ref, msgsender_MSG: Ref, msgvalue_MSG: int, mode_s146: int)
 {
 
   anon0:
-    call {:si_unique_call 35} {:cexpr "_verisolFirstArg"} boogie_si_record_sol2Bpl_bool(false);
-    call {:si_unique_call 36} {:cexpr "this"} boogie_si_record_sol2Bpl_ref(this);
-    call {:si_unique_call 37} {:cexpr "msg.sender"} boogie_si_record_sol2Bpl_ref(msgsender_MSG);
-    call {:si_unique_call 38} {:cexpr "msg.value"} boogie_si_record_sol2Bpl_int(msgvalue_MSG);
-    call {:si_unique_call 39} {:cexpr "_verisolLastArg"} boogie_si_record_sol2Bpl_bool(true);
+    call {:si_unique_call 36} {:cexpr "_verisolFirstArg"} boogie_si_record_sol2Bpl_bool(false);
+    call {:si_unique_call 37} {:cexpr "this"} boogie_si_record_sol2Bpl_ref(this);
+    call {:si_unique_call 38} {:cexpr "msg.sender"} boogie_si_record_sol2Bpl_ref(msgsender_MSG);
+    call {:si_unique_call 39} {:cexpr "msg.value"} boogie_si_record_sol2Bpl_int(msgvalue_MSG);
+    call {:si_unique_call 40} {:cexpr "_verisolLastArg"} boogie_si_record_sol2Bpl_bool(true);
+    goto corral_source_split_23;
+
+  corral_source_split_23:
+    goto corral_source_split_24;
+
+  corral_source_split_24:
+    goto anon3_Then, anon3_Else;
+
+  anon3_Then:
+    assume {:partition} User_RoomThermostat[this] != msgsender_MSG || State_RoomThermostat[this] != 1;
     goto corral_source_split_26;
 
   corral_source_split_26:
     goto corral_source_split_27;
 
   corral_source_split_27:
-    goto anon5_Then, anon5_Else;
-
-  anon5_Then:
-    assume {:partition} StateEnum_SimpleMarketplace[this] != 1;
-    goto corral_source_split_29;
-
-  corral_source_split_29:
-    goto corral_source_split_30;
-
-  corral_source_split_30:
     assume false;
     goto anon2;
 
-  anon5_Else:
-    assume {:partition} StateEnum_SimpleMarketplace[this] == 1;
+  anon3_Else:
+    assume {:partition} !(User_RoomThermostat[this] != msgsender_MSG || State_RoomThermostat[this] != 1);
     goto anon2;
 
   anon2:
-    goto anon6_Then, anon6_Else;
-
-  anon6_Then:
-    assume {:partition} InstanceOwner_SimpleMarketplace[this] != msgsender_MSG;
-    goto corral_source_split_32;
-
-  corral_source_split_32:
-    goto corral_source_split_33;
-
-  corral_source_split_33:
-    assume false;
-    goto anon4;
-
-  anon6_Else:
-    assume {:partition} InstanceOwner_SimpleMarketplace[this] == msgsender_MSG;
-    goto anon4;
-
-  anon4:
-    StateEnum_SimpleMarketplace[this] := 0;
-    return;
-}
-
-
-
-procedure {:public} AcceptOffer_SimpleMarketplace(this: Ref, msgsender_MSG: Ref, msgvalue_MSG: int);
-  modifies StateEnum_SimpleMarketplace;
-
-
-
-implementation {:ForceInline} AcceptOffer_SimpleMarketplace(this: Ref, msgsender_MSG: Ref, msgvalue_MSG: int)
-{
-
-  anon0:
-    call {:si_unique_call 40} {:cexpr "_verisolFirstArg"} boogie_si_record_sol2Bpl_bool(false);
-    call {:si_unique_call 41} {:cexpr "this"} boogie_si_record_sol2Bpl_ref(this);
-    call {:si_unique_call 42} {:cexpr "msg.sender"} boogie_si_record_sol2Bpl_ref(msgsender_MSG);
-    call {:si_unique_call 43} {:cexpr "msg.value"} boogie_si_record_sol2Bpl_int(msgvalue_MSG);
-    call {:si_unique_call 44} {:cexpr "_verisolLastArg"} boogie_si_record_sol2Bpl_bool(true);
-    goto corral_source_split_35;
-
-  corral_source_split_35:
-    goto corral_source_split_36;
-
-  corral_source_split_36:
-    goto anon5_Then, anon5_Else;
-
-  anon5_Then:
-    assume {:partition} StateEnum_SimpleMarketplace[this] != 1;
-    goto corral_source_split_38;
-
-  corral_source_split_38:
-    goto corral_source_split_39;
-
-  corral_source_split_39:
-    assume false;
-    goto anon2;
-
-  anon5_Else:
-    assume {:partition} StateEnum_SimpleMarketplace[this] == 1;
-    goto anon2;
-
-  anon2:
-    goto anon6_Then, anon6_Else;
-
-  anon6_Then:
-    assume {:partition} msgsender_MSG != InstanceOwner_SimpleMarketplace[this];
-    goto corral_source_split_41;
-
-  corral_source_split_41:
-    goto corral_source_split_42;
-
-  corral_source_split_42:
-    assume false;
-    goto anon4;
-
-  anon6_Else:
-    assume {:partition} msgsender_MSG == InstanceOwner_SimpleMarketplace[this];
-    goto anon4;
-
-  anon4:
-    StateEnum_SimpleMarketplace[this] := 2;
+    Mode_RoomThermostat[this] := mode_s146;
     return;
 }
 
@@ -440,60 +342,62 @@ procedure send(from: Ref, to: Ref, amount: int) returns (success: bool);
 
 
 
-const {:existential true} HoudiniB1_SimpleMarketplace: bool;
+const {:existential true} HoudiniB1_RoomThermostat: bool;
 
-const {:existential true} HoudiniB2_SimpleMarketplace: bool;
+const {:existential true} HoudiniB2_RoomThermostat: bool;
 
-const {:existential true} HoudiniB3_SimpleMarketplace: bool;
+const {:existential true} HoudiniB3_RoomThermostat: bool;
 
-const {:existential true} HoudiniB4_SimpleMarketplace: bool;
+const {:existential true} HoudiniB4_RoomThermostat: bool;
 
-const {:existential true} HoudiniB5_SimpleMarketplace: bool;
+const {:existential true} HoudiniB5_RoomThermostat: bool;
 
-const {:existential true} HoudiniB6_SimpleMarketplace: bool;
+const {:existential true} HoudiniB6_RoomThermostat: bool;
 
-procedure BoogieEntry_SimpleMarketplace();
-
-
-
-procedure CorralChoice_SimpleMarketplace(this: Ref);
-  modifies now, Alloc, InstanceBuyer_SimpleMarketplace, OfferPrice_SimpleMarketplace, StateEnum_SimpleMarketplace;
+procedure BoogieEntry_RoomThermostat();
 
 
 
-implementation CorralChoice_SimpleMarketplace(this: Ref)
+procedure CorralChoice_RoomThermostat(this: Ref);
+  modifies now, Alloc, State_RoomThermostat, TargetTemperature_RoomThermostat, Mode_RoomThermostat;
+
+
+
+implementation CorralChoice_RoomThermostat(this: Ref)
 {
   var msgsender_MSG: Ref;
   var msgvalue_MSG: int;
   var choice: int;
-  var offerPrice_s31: int;
-  var description_s78: int;
-  var price_s78: int;
-  var sender_s78: Ref;
-  var offerPrice_s124: int;
+  var targetTemperature_s32: int;
+  var mode_s32: int;
+  var thermostatInstaller_s75: Ref;
+  var thermostatUser_s75: Ref;
+  var targetTemperature_s122: int;
+  var mode_s146: int;
   var tmpNow: int;
 
   anon0:
     havoc msgsender_MSG;
     havoc msgvalue_MSG;
     havoc choice;
-    havoc offerPrice_s31;
-    havoc description_s78;
-    havoc price_s78;
-    havoc sender_s78;
-    havoc offerPrice_s124;
+    havoc targetTemperature_s32;
+    havoc mode_s32;
+    havoc thermostatInstaller_s75;
+    havoc thermostatUser_s75;
+    havoc targetTemperature_s122;
+    havoc mode_s146;
     havoc tmpNow;
     tmpNow := now;
     havoc now;
     assume now > tmpNow;
     assume msgsender_MSG != null;
-    assume DType[msgsender_MSG] != SimpleMarketplace;
+    assume DType[msgsender_MSG] != RoomThermostat;
     Alloc[msgsender_MSG] := true;
     goto anon5_Then, anon5_Else;
 
   anon5_Then:
     assume {:partition} choice == 4;
-    call {:si_unique_call 45} prueba_SimpleMarketplace(this, msgsender_MSG, msgvalue_MSG, offerPrice_s31);
+    call {:si_unique_call 41} prueba_RoomThermostat(this, msgsender_MSG, msgvalue_MSG, targetTemperature_s32, mode_s32);
     return;
 
   anon5_Else:
@@ -502,7 +406,7 @@ implementation CorralChoice_SimpleMarketplace(this: Ref)
 
   anon6_Then:
     assume {:partition} choice == 3;
-    call {:si_unique_call 46} MakeOffer_SimpleMarketplace(this, msgsender_MSG, msgvalue_MSG, offerPrice_s124);
+    call {:si_unique_call 42} StartThermostat_RoomThermostat(this, msgsender_MSG, msgvalue_MSG);
     return;
 
   anon6_Else:
@@ -511,7 +415,7 @@ implementation CorralChoice_SimpleMarketplace(this: Ref)
 
   anon7_Then:
     assume {:partition} choice == 2;
-    call {:si_unique_call 47} Reject_SimpleMarketplace(this, msgsender_MSG, msgvalue_MSG);
+    call {:si_unique_call 43} SetTargetTemperature_RoomThermostat(this, msgsender_MSG, msgvalue_MSG, targetTemperature_s122);
     return;
 
   anon7_Else:
@@ -520,7 +424,7 @@ implementation CorralChoice_SimpleMarketplace(this: Ref)
 
   anon8_Then:
     assume {:partition} choice == 1;
-    call {:si_unique_call 48} AcceptOffer_SimpleMarketplace(this, msgsender_MSG, msgvalue_MSG);
+    call {:si_unique_call 44} SetMode_RoomThermostat(this, msgsender_MSG, msgvalue_MSG, mode_s146);
     return;
 
   anon8_Else:
@@ -530,25 +434,24 @@ implementation CorralChoice_SimpleMarketplace(this: Ref)
 
 
 
-procedure CorralEntry_SimpleMarketplace();
-  modifies Alloc, Balance, InstanceOwner_SimpleMarketplace, Description_SimpleMarketplace, AskingPrice_SimpleMarketplace, result_SimpleMarketplace, InstanceBuyer_SimpleMarketplace, OfferPrice_SimpleMarketplace, StateEnum_SimpleMarketplace, now;
+procedure CorralEntry_RoomThermostat();
+  modifies Alloc, Balance, Installer_RoomThermostat, User_RoomThermostat, TargetTemperature_RoomThermostat, State_RoomThermostat, now, Mode_RoomThermostat;
 
 
 
-implementation CorralEntry_SimpleMarketplace()
+implementation CorralEntry_RoomThermostat()
 {
   var this: Ref;
   var msgsender_MSG: Ref;
   var msgvalue_MSG: int;
-  var description_s78: int;
-  var price_s78: int;
-  var sender_s78: Ref;
+  var thermostatInstaller_s75: Ref;
+  var thermostatUser_s75: Ref;
 
   anon0:
-    call {:si_unique_call 49} this := FreshRefGenerator();
+    call {:si_unique_call 45} this := FreshRefGenerator();
     assume now >= 0;
-    assume DType[this] == SimpleMarketplace;
-    call {:si_unique_call 50} SimpleMarketplace_SimpleMarketplace(this, msgsender_MSG, msgvalue_MSG, description_s78, price_s78, sender_s78);
+    assume DType[this] == RoomThermostat;
+    call {:si_unique_call 46} RoomThermostat_RoomThermostat(this, msgsender_MSG, msgvalue_MSG, thermostatInstaller_s75, thermostatUser_s75);
     goto anon2_LoopHead;
 
   anon2_LoopHead:
@@ -556,7 +459,7 @@ implementation CorralEntry_SimpleMarketplace()
 
   anon2_LoopBody:
     assume {:partition} true;
-    call {:si_unique_call 51} CorralChoice_SimpleMarketplace(this);
+    call {:si_unique_call 47} CorralChoice_RoomThermostat(this);
     goto anon2_LoopHead;
 
   anon2_LoopDone:
