2/new_folder4/__SolToBoogieTest_out.bpl
@@ -1,7 +1,7 @@
 type Ref;
 type ContractName;
 const unique null: Ref;
-const unique SimpleMarketplace: ContractName;
+const unique AssetTransfer: ContractName;
 function ConstantToRef(x: int) returns (ret: Ref);
 function BoogieRefToInt(x: Ref) returns (ret: int);
 function {:bvbuiltin "mod"} modBpl(x: int, y: int) returns (ret: int);
@@ -15,8 +15,6 @@ var Balance: [Ref]int;
 var DType: [Ref]ContractName;
 var Alloc: [Ref]bool;
 var balance_ADDR: [Ref]int;
-var M_int_int: [Ref][int]int;
-var M_int_Ref: [Ref][int]Ref;
 var Length: [Ref]int;
 var now: int;
 procedure {:inline 1} FreshRefGenerator() returns (newRef: Ref);
@@ -56,175 +54,441 @@ axiom(forall  __i__0_0:int, __i__0_1:int, __i__1_0:int, __i__1_1:int :: {abiEnco
 axiom(forall  __i__0_0:Ref, __i__0_1:Ref :: {abiEncodePacked1R(__i__0_0), abiEncodePacked1R(__i__0_1)} (((__i__0_0) == (__i__0_1)) || ((abiEncodePacked1R(__i__0_0)) != (abiEncodePacked1R(__i__0_1)))));
 
 axiom(forall  __i__0_0:Ref, __i__0_1:Ref, __i__1_0:int, __i__1_1:int :: {abiEncodePacked2R(__i__0_0, __i__1_0), abiEncodePacked2R(__i__0_1, __i__1_1)} ((((__i__0_0) == (__i__0_1)) && ((__i__1_0) == (__i__1_1))) || ((abiEncodePacked2R(__i__0_0, __i__1_0)) != (abiEncodePacked2R(__i__0_1, __i__1_1)))));
-procedure {:public} {:inline 1} prueba_SimpleMarketplace(this: Ref, msgsender_MSG: Ref, msgvalue_MSG: int, offerPrice_s31: int);
-implementation prueba_SimpleMarketplace(this: Ref, msgsender_MSG: Ref, msgvalue_MSG: int, offerPrice_s31: int)
+procedure {:public} {:inline 1} prueba_AssetTransfer(this: Ref, msgsender_MSG: Ref, msgvalue_MSG: int, offerPrice_s143: int, inspector_s143: Ref, appraiser_s143: Ref, description_s143: int, price_s143: int);
+implementation prueba_AssetTransfer(this: Ref, msgsender_MSG: Ref, msgvalue_MSG: int, offerPrice_s143: int, inspector_s143: Ref, appraiser_s143: Ref, description_s143: int, price_s143: int)
 {
 call  {:cexpr "_verisolFirstArg"} boogie_si_record_sol2Bpl_bool(false);
 call  {:cexpr "this"} boogie_si_record_sol2Bpl_ref(this);
 call  {:cexpr "msg.sender"} boogie_si_record_sol2Bpl_ref(msgsender_MSG);
 call  {:cexpr "msg.value"} boogie_si_record_sol2Bpl_int(msgvalue_MSG);
-call  {:cexpr "offerPrice"} boogie_si_record_sol2Bpl_int(offerPrice_s31);
+call  {:cexpr "offerPrice"} boogie_si_record_sol2Bpl_int(offerPrice_s143);
+call  {:cexpr "inspector"} boogie_si_record_sol2Bpl_ref(inspector_s143);
+call  {:cexpr "appraiser"} boogie_si_record_sol2Bpl_ref(appraiser_s143);
+call  {:cexpr "description"} boogie_si_record_sol2Bpl_int(description_s143);
+call  {:cexpr "price"} boogie_si_record_sol2Bpl_int(price_s143);
 call  {:cexpr "_verisolLastArg"} boogie_si_record_sol2Bpl_bool(true);
-assert {:first} {:sourceFile "/Users/etorres/Proyectos/verisol-test/2/new_folder4/CombinationsTemp4.sol"} {:sourceLine 5} (true);
+assert {:first} {:sourceFile "/Users/etorres/Proyectos/verisol-test/2/new_folder4/CombinationsTemp4.sol"} {:sourceLine 4} (true);
+assert {:first} {:sourceFile "/Users/etorres/Proyectos/verisol-test/2/new_folder4/CombinationsTemp4.sol"} {:sourceLine 6} (true);
+assume ((((((((((!((true))) && (!(((State_AssetTransfer[this]) == (0))))) && ((State_AssetTransfer[this]) == (0))) && ((State_AssetTransfer[this]) == (1))) && (!(((((((State_AssetTransfer[this]) == (1)) || ((State_AssetTransfer[this]) == (2))) || ((State_AssetTransfer[this]) == (3))) || (((State_AssetTransfer[this]) == (4)) && ((State_AssetTransfer[this]) == (5)))) || ((State_AssetTransfer[this]) == (6)))))) && (true)) && (!(((State_AssetTransfer[this]) == (1))))) && (!((((((((State_AssetTransfer[this]) == (1)) || ((State_AssetTransfer[this]) == (2))) || ((State_AssetTransfer[this]) == (3))) || ((State_AssetTransfer[this]) == (4))) || ((State_AssetTransfer[this]) == (5))) || ((State_AssetTransfer[this]) == (7)))))) && (!((((State_AssetTransfer[this]) != (2)) || ((State_AssetTransfer[this]) != (3)))))) && (!((((State_AssetTransfer[this]) != (2)) || ((State_AssetTransfer[this]) != (4))))));
 assert {:first} {:sourceFile "/Users/etorres/Proyectos/verisol-test/2/new_folder4/CombinationsTemp4.sol"} {:sourceLine 7} (true);
-assume ((((StateEnum_SimpleMarketplace[this]) == (0)) && ((StateEnum_SimpleMarketplace[this]) == (1))) && (!(((StateEnum_SimpleMarketplace[this]) == (1)))));
-assert {:first} {:sourceFile "/Users/etorres/Proyectos/verisol-test/2/new_folder4/CombinationsTemp4.sol"} {:sourceLine 8} (true);
 assert (false);
 }
 
-var InstanceOwner_SimpleMarketplace: [Ref]Ref;
-var Description_SimpleMarketplace: [Ref]int;
-var AskingPrice_SimpleMarketplace: [Ref]int;
-var StateEnum_SimpleMarketplace: [Ref]int;
-var result_SimpleMarketplace: [Ref]Ref;
-var InstanceBuyer_SimpleMarketplace: [Ref]Ref;
-var OfferPrice_SimpleMarketplace: [Ref]int;
-procedure {:inline 1} SimpleMarketplace_SimpleMarketplace_NoBaseCtor(this: Ref, msgsender_MSG: Ref, msgvalue_MSG: int, description_s78: int, price_s78: int, sender_s78: Ref);
-implementation SimpleMarketplace_SimpleMarketplace_NoBaseCtor(this: Ref, msgsender_MSG: Ref, msgvalue_MSG: int, description_s78: int, price_s78: int, sender_s78: Ref)
+var InstanceOwner_AssetTransfer: [Ref]Ref;
+var Description_AssetTransfer: [Ref]int;
+var AskingPrice_AssetTransfer: [Ref]int;
+var State_AssetTransfer: [Ref]int;
+var InstanceBuyer_AssetTransfer: [Ref]Ref;
+var OfferPrice_AssetTransfer: [Ref]int;
+var InstanceInspector_AssetTransfer: [Ref]Ref;
+var InstanceAppraiser_AssetTransfer: [Ref]Ref;
+procedure {:inline 1} AssetTransfer_AssetTransfer_NoBaseCtor(this: Ref, msgsender_MSG: Ref, msgvalue_MSG: int, description_s196: int, price_s196: int);
+implementation AssetTransfer_AssetTransfer_NoBaseCtor(this: Ref, msgsender_MSG: Ref, msgvalue_MSG: int, description_s196: int, price_s196: int)
 {
-var __var_1: Ref;
 // start of initialization
 assume ((msgsender_MSG) != (null));
 Balance[this] := 0;
-InstanceOwner_SimpleMarketplace[this] := null;
-Description_SimpleMarketplace[this] := -1504705494;
-AskingPrice_SimpleMarketplace[this] := 0;
-// Make array/mapping vars distinct for result
-call __var_1 := FreshRefGenerator();
-result_SimpleMarketplace[this] := __var_1;
-assume ((Length[result_SimpleMarketplace[this]]) == (0));
-InstanceBuyer_SimpleMarketplace[this] := null;
-OfferPrice_SimpleMarketplace[this] := 0;
+InstanceOwner_AssetTransfer[this] := null;
+Description_AssetTransfer[this] := -1653894714;
+AskingPrice_AssetTransfer[this] := 0;
+InstanceBuyer_AssetTransfer[this] := null;
+OfferPrice_AssetTransfer[this] := 0;
+InstanceInspector_AssetTransfer[this] := null;
+InstanceAppraiser_AssetTransfer[this] := null;
 // end of initialization
 call  {:cexpr "_verisolFirstArg"} boogie_si_record_sol2Bpl_bool(false);
 call  {:cexpr "this"} boogie_si_record_sol2Bpl_ref(this);
 call  {:cexpr "msg.sender"} boogie_si_record_sol2Bpl_ref(msgsender_MSG);
 call  {:cexpr "msg.value"} boogie_si_record_sol2Bpl_int(msgvalue_MSG);
-call  {:cexpr "description"} boogie_si_record_sol2Bpl_int(description_s78);
-call  {:cexpr "price"} boogie_si_record_sol2Bpl_int(price_s78);
-call  {:cexpr "sender"} boogie_si_record_sol2Bpl_ref(sender_s78);
+call  {:cexpr "description"} boogie_si_record_sol2Bpl_int(description_s196);
+call  {:cexpr "price"} boogie_si_record_sol2Bpl_int(price_s196);
 call  {:cexpr "_verisolLastArg"} boogie_si_record_sol2Bpl_bool(true);
-assert {:first} {:sourceFile "/Users/etorres/Proyectos/verisol-test/2/new_folder4/CombinationsTemp4.sol"} {:sourceLine 28} (true);
-assert {:first} {:sourceFile "/Users/etorres/Proyectos/verisol-test/2/new_folder4/CombinationsTemp4.sol"} {:sourceLine 29} (true);
-InstanceOwner_SimpleMarketplace[this] := sender_s78;
-call  {:cexpr "InstanceOwner"} boogie_si_record_sol2Bpl_ref(InstanceOwner_SimpleMarketplace[this]);
-assert {:first} {:sourceFile "/Users/etorres/Proyectos/verisol-test/2/new_folder4/CombinationsTemp4.sol"} {:sourceLine 30} (true);
-AskingPrice_SimpleMarketplace[this] := price_s78;
-call  {:cexpr "AskingPrice"} boogie_si_record_sol2Bpl_int(AskingPrice_SimpleMarketplace[this]);
-assert {:first} {:sourceFile "/Users/etorres/Proyectos/verisol-test/2/new_folder4/CombinationsTemp4.sol"} {:sourceLine 31} (true);
-Description_SimpleMarketplace[this] := description_s78;
-call  {:cexpr "Description"} boogie_si_record_sol2Bpl_int(Description_SimpleMarketplace[this]);
+assert {:first} {:sourceFile "/Users/etorres/Proyectos/verisol-test/2/new_folder4/CombinationsTemp4.sol"} {:sourceLine 23} (true);
+assert {:first} {:sourceFile "/Users/etorres/Proyectos/verisol-test/2/new_folder4/CombinationsTemp4.sol"} {:sourceLine 24} (true);
+InstanceOwner_AssetTransfer[this] := msgsender_MSG;
+call  {:cexpr "InstanceOwner"} boogie_si_record_sol2Bpl_ref(InstanceOwner_AssetTransfer[this]);
+assert {:first} {:sourceFile "/Users/etorres/Proyectos/verisol-test/2/new_folder4/CombinationsTemp4.sol"} {:sourceLine 25} (true);
+assume ((AskingPrice_AssetTransfer[this]) >= (0));
+assume ((price_s196) >= (0));
+AskingPrice_AssetTransfer[this] := price_s196;
+call  {:cexpr "AskingPrice"} boogie_si_record_sol2Bpl_int(AskingPrice_AssetTransfer[this]);
+assert {:first} {:sourceFile "/Users/etorres/Proyectos/verisol-test/2/new_folder4/CombinationsTemp4.sol"} {:sourceLine 26} (true);
+Description_AssetTransfer[this] := description_s196;
+call  {:cexpr "Description"} boogie_si_record_sol2Bpl_int(Description_AssetTransfer[this]);
+assert {:first} {:sourceFile "/Users/etorres/Proyectos/verisol-test/2/new_folder4/CombinationsTemp4.sol"} {:sourceLine 27} (true);
+State_AssetTransfer[this] := 0;
+}
+
+procedure {:constructor} {:public} {:inline 1} AssetTransfer_AssetTransfer(this: Ref, msgsender_MSG: Ref, msgvalue_MSG: int, description_s196: int, price_s196: int);
+implementation AssetTransfer_AssetTransfer(this: Ref, msgsender_MSG: Ref, msgvalue_MSG: int, description_s196: int, price_s196: int)
+{
+call  {:cexpr "_verisolFirstArg"} boogie_si_record_sol2Bpl_bool(false);
+call  {:cexpr "this"} boogie_si_record_sol2Bpl_ref(this);
+call  {:cexpr "msg.sender"} boogie_si_record_sol2Bpl_ref(msgsender_MSG);
+call  {:cexpr "msg.value"} boogie_si_record_sol2Bpl_int(msgvalue_MSG);
+call  {:cexpr "description"} boogie_si_record_sol2Bpl_int(description_s196);
+call  {:cexpr "price"} boogie_si_record_sol2Bpl_int(price_s196);
+call  {:cexpr "_verisolLastArg"} boogie_si_record_sol2Bpl_bool(true);
+call AssetTransfer_AssetTransfer_NoBaseCtor(this, msgsender_MSG, msgvalue_MSG, description_s196, price_s196);
+}
+
+procedure {:public} {:inline 1} Terminate_AssetTransfer(this: Ref, msgsender_MSG: Ref, msgvalue_MSG: int);
+implementation Terminate_AssetTransfer(this: Ref, msgsender_MSG: Ref, msgvalue_MSG: int)
+{
+call  {:cexpr "_verisolFirstArg"} boogie_si_record_sol2Bpl_bool(false);
+call  {:cexpr "this"} boogie_si_record_sol2Bpl_ref(this);
+call  {:cexpr "msg.sender"} boogie_si_record_sol2Bpl_ref(msgsender_MSG);
+call  {:cexpr "msg.value"} boogie_si_record_sol2Bpl_int(msgvalue_MSG);
+call  {:cexpr "_verisolLastArg"} boogie_si_record_sol2Bpl_bool(true);
 assert {:first} {:sourceFile "/Users/etorres/Proyectos/verisol-test/2/new_folder4/CombinationsTemp4.sol"} {:sourceLine 32} (true);
-StateEnum_SimpleMarketplace[this] := 0;
-}
-
-procedure {:constructor} {:public} {:inline 1} SimpleMarketplace_SimpleMarketplace(this: Ref, msgsender_MSG: Ref, msgvalue_MSG: int, description_s78: int, price_s78: int, sender_s78: Ref);
-implementation SimpleMarketplace_SimpleMarketplace(this: Ref, msgsender_MSG: Ref, msgvalue_MSG: int, description_s78: int, price_s78: int, sender_s78: Ref)
-{
-var __var_1: Ref;
-call  {:cexpr "_verisolFirstArg"} boogie_si_record_sol2Bpl_bool(false);
-call  {:cexpr "this"} boogie_si_record_sol2Bpl_ref(this);
-call  {:cexpr "msg.sender"} boogie_si_record_sol2Bpl_ref(msgsender_MSG);
-call  {:cexpr "msg.value"} boogie_si_record_sol2Bpl_int(msgvalue_MSG);
-call  {:cexpr "description"} boogie_si_record_sol2Bpl_int(description_s78);
-call  {:cexpr "price"} boogie_si_record_sol2Bpl_int(price_s78);
-call  {:cexpr "sender"} boogie_si_record_sol2Bpl_ref(sender_s78);
-call  {:cexpr "_verisolLastArg"} boogie_si_record_sol2Bpl_bool(true);
-call SimpleMarketplace_SimpleMarketplace_NoBaseCtor(this, msgsender_MSG, msgvalue_MSG, description_s78, price_s78, sender_s78);
-}
-
-procedure {:public} {:inline 1} MakeOffer_SimpleMarketplace(this: Ref, msgsender_MSG: Ref, msgvalue_MSG: int, offerPrice_s124: int);
-implementation MakeOffer_SimpleMarketplace(this: Ref, msgsender_MSG: Ref, msgvalue_MSG: int, offerPrice_s124: int)
-{
-call  {:cexpr "_verisolFirstArg"} boogie_si_record_sol2Bpl_bool(false);
-call  {:cexpr "this"} boogie_si_record_sol2Bpl_ref(this);
-call  {:cexpr "msg.sender"} boogie_si_record_sol2Bpl_ref(msgsender_MSG);
-call  {:cexpr "msg.value"} boogie_si_record_sol2Bpl_int(msgvalue_MSG);
-call  {:cexpr "offerPrice"} boogie_si_record_sol2Bpl_int(offerPrice_s124);
-call  {:cexpr "_verisolLastArg"} boogie_si_record_sol2Bpl_bool(true);
-assert {:first} {:sourceFile "/Users/etorres/Proyectos/verisol-test/2/new_folder4/CombinationsTemp4.sol"} {:sourceLine 36} (true);
-assert {:first} {:sourceFile "/Users/etorres/Proyectos/verisol-test/2/new_folder4/CombinationsTemp4.sol"} {:sourceLine 37} (true);
-if ((offerPrice_s124) == (0)) {
-assert {:first} {:sourceFile "/Users/etorres/Proyectos/verisol-test/2/new_folder4/CombinationsTemp4.sol"} {:sourceLine 38} (true);
-assert {:first} {:sourceFile "/Users/etorres/Proyectos/verisol-test/2/new_folder4/CombinationsTemp4.sol"} {:sourceLine 39} (true);
+assert {:first} {:sourceFile "/Users/etorres/Proyectos/verisol-test/2/new_folder4/CombinationsTemp4.sol"} {:sourceLine 33} (true);
+if ((InstanceOwner_AssetTransfer[this]) != (msgsender_MSG)) {
+assert {:first} {:sourceFile "/Users/etorres/Proyectos/verisol-test/2/new_folder4/CombinationsTemp4.sol"} {:sourceLine 34} (true);
+assert {:first} {:sourceFile "/Users/etorres/Proyectos/verisol-test/2/new_folder4/CombinationsTemp4.sol"} {:sourceLine 35} (true);
 assume (false);
 }
-assert {:first} {:sourceFile "/Users/etorres/Proyectos/verisol-test/2/new_folder4/CombinationsTemp4.sol"} {:sourceLine 42} (true);
-if ((StateEnum_SimpleMarketplace[this]) != (0)) {
+assert {:first} {:sourceFile "/Users/etorres/Proyectos/verisol-test/2/new_folder4/CombinationsTemp4.sol"} {:sourceLine 38} (true);
+State_AssetTransfer[this] := 9;
+}
+
+procedure {:public} {:inline 1} Modify_AssetTransfer(this: Ref, msgsender_MSG: Ref, msgvalue_MSG: int, description_s248: int, price_s248: int);
+implementation Modify_AssetTransfer(this: Ref, msgsender_MSG: Ref, msgvalue_MSG: int, description_s248: int, price_s248: int)
+{
+call  {:cexpr "_verisolFirstArg"} boogie_si_record_sol2Bpl_bool(false);
+call  {:cexpr "this"} boogie_si_record_sol2Bpl_ref(this);
+call  {:cexpr "msg.sender"} boogie_si_record_sol2Bpl_ref(msgsender_MSG);
+call  {:cexpr "msg.value"} boogie_si_record_sol2Bpl_int(msgvalue_MSG);
+call  {:cexpr "description"} boogie_si_record_sol2Bpl_int(description_s248);
+call  {:cexpr "price"} boogie_si_record_sol2Bpl_int(price_s248);
+call  {:cexpr "_verisolLastArg"} boogie_si_record_sol2Bpl_bool(true);
 assert {:first} {:sourceFile "/Users/etorres/Proyectos/verisol-test/2/new_folder4/CombinationsTemp4.sol"} {:sourceLine 43} (true);
 assert {:first} {:sourceFile "/Users/etorres/Proyectos/verisol-test/2/new_folder4/CombinationsTemp4.sol"} {:sourceLine 44} (true);
+if ((State_AssetTransfer[this]) != (0)) {
+assert {:first} {:sourceFile "/Users/etorres/Proyectos/verisol-test/2/new_folder4/CombinationsTemp4.sol"} {:sourceLine 45} (true);
+assert {:first} {:sourceFile "/Users/etorres/Proyectos/verisol-test/2/new_folder4/CombinationsTemp4.sol"} {:sourceLine 46} (true);
 assume (false);
 }
-assert {:first} {:sourceFile "/Users/etorres/Proyectos/verisol-test/2/new_folder4/CombinationsTemp4.sol"} {:sourceLine 47} (true);
-if ((InstanceOwner_SimpleMarketplace[this]) == (msgsender_MSG)) {
 assert {:first} {:sourceFile "/Users/etorres/Proyectos/verisol-test/2/new_folder4/CombinationsTemp4.sol"} {:sourceLine 48} (true);
+if ((InstanceOwner_AssetTransfer[this]) != (msgsender_MSG)) {
 assert {:first} {:sourceFile "/Users/etorres/Proyectos/verisol-test/2/new_folder4/CombinationsTemp4.sol"} {:sourceLine 49} (true);
+assert {:first} {:sourceFile "/Users/etorres/Proyectos/verisol-test/2/new_folder4/CombinationsTemp4.sol"} {:sourceLine 50} (true);
 assume (false);
 }
-assert {:first} {:sourceFile "/Users/etorres/Proyectos/verisol-test/2/new_folder4/CombinationsTemp4.sol"} {:sourceLine 52} (true);
-InstanceBuyer_SimpleMarketplace[this] := msgsender_MSG;
-call  {:cexpr "InstanceBuyer"} boogie_si_record_sol2Bpl_ref(InstanceBuyer_SimpleMarketplace[this]);
 assert {:first} {:sourceFile "/Users/etorres/Proyectos/verisol-test/2/new_folder4/CombinationsTemp4.sol"} {:sourceLine 53} (true);
-OfferPrice_SimpleMarketplace[this] := offerPrice_s124;
-call  {:cexpr "OfferPrice"} boogie_si_record_sol2Bpl_int(OfferPrice_SimpleMarketplace[this]);
+Description_AssetTransfer[this] := description_s248;
+call  {:cexpr "Description"} boogie_si_record_sol2Bpl_int(Description_AssetTransfer[this]);
 assert {:first} {:sourceFile "/Users/etorres/Proyectos/verisol-test/2/new_folder4/CombinationsTemp4.sol"} {:sourceLine 54} (true);
-StateEnum_SimpleMarketplace[this] := 1;
+assume ((AskingPrice_AssetTransfer[this]) >= (0));
+assume ((price_s248) >= (0));
+AskingPrice_AssetTransfer[this] := price_s248;
+call  {:cexpr "AskingPrice"} boogie_si_record_sol2Bpl_int(AskingPrice_AssetTransfer[this]);
 }
 
-procedure {:public} {:inline 1} Reject_SimpleMarketplace(this: Ref, msgsender_MSG: Ref, msgvalue_MSG: int);
-implementation Reject_SimpleMarketplace(this: Ref, msgsender_MSG: Ref, msgvalue_MSG: int)
+procedure {:public} {:inline 1} MakeOffer_AssetTransfer(this: Ref, msgsender_MSG: Ref, msgvalue_MSG: int, inspector_s318: Ref, appraiser_s318: Ref, offerPrice_s318: int);
+implementation MakeOffer_AssetTransfer(this: Ref, msgsender_MSG: Ref, msgvalue_MSG: int, inspector_s318: Ref, appraiser_s318: Ref, offerPrice_s318: int)
 {
+var __var_1: Ref;
+var __var_2: Ref;
 call  {:cexpr "_verisolFirstArg"} boogie_si_record_sol2Bpl_bool(false);
 call  {:cexpr "this"} boogie_si_record_sol2Bpl_ref(this);
 call  {:cexpr "msg.sender"} boogie_si_record_sol2Bpl_ref(msgsender_MSG);
 call  {:cexpr "msg.value"} boogie_si_record_sol2Bpl_int(msgvalue_MSG);
+call  {:cexpr "inspector"} boogie_si_record_sol2Bpl_ref(inspector_s318);
+call  {:cexpr "appraiser"} boogie_si_record_sol2Bpl_ref(appraiser_s318);
+call  {:cexpr "offerPrice"} boogie_si_record_sol2Bpl_int(offerPrice_s318);
 call  {:cexpr "_verisolLastArg"} boogie_si_record_sol2Bpl_bool(true);
-assert {:first} {:sourceFile "/Users/etorres/Proyectos/verisol-test/2/new_folder4/CombinationsTemp4.sol"} {:sourceLine 58} (true);
 assert {:first} {:sourceFile "/Users/etorres/Proyectos/verisol-test/2/new_folder4/CombinationsTemp4.sol"} {:sourceLine 59} (true);
-if ((StateEnum_SimpleMarketplace[this]) != (1)) {
 assert {:first} {:sourceFile "/Users/etorres/Proyectos/verisol-test/2/new_folder4/CombinationsTemp4.sol"} {:sourceLine 60} (true);
+__var_1 := null;
+__var_2 := null;
+assume ((offerPrice_s318) >= (0));
+if ((((inspector_s318) == (null)) || ((appraiser_s318) == (null))) || ((offerPrice_s318) == (0))) {
 assert {:first} {:sourceFile "/Users/etorres/Proyectos/verisol-test/2/new_folder4/CombinationsTemp4.sol"} {:sourceLine 61} (true);
+assert {:first} {:sourceFile "/Users/etorres/Proyectos/verisol-test/2/new_folder4/CombinationsTemp4.sol"} {:sourceLine 62} (true);
 assume (false);
 }
 assert {:first} {:sourceFile "/Users/etorres/Proyectos/verisol-test/2/new_folder4/CombinationsTemp4.sol"} {:sourceLine 64} (true);
-if ((InstanceOwner_SimpleMarketplace[this]) != (msgsender_MSG)) {
+if ((State_AssetTransfer[this]) != (0)) {
 assert {:first} {:sourceFile "/Users/etorres/Proyectos/verisol-test/2/new_folder4/CombinationsTemp4.sol"} {:sourceLine 65} (true);
 assert {:first} {:sourceFile "/Users/etorres/Proyectos/verisol-test/2/new_folder4/CombinationsTemp4.sol"} {:sourceLine 66} (true);
 assume (false);
 }
+assert {:first} {:sourceFile "/Users/etorres/Proyectos/verisol-test/2/new_folder4/CombinationsTemp4.sol"} {:sourceLine 69} (true);
+if ((InstanceOwner_AssetTransfer[this]) == (msgsender_MSG)) {
 assert {:first} {:sourceFile "/Users/etorres/Proyectos/verisol-test/2/new_folder4/CombinationsTemp4.sol"} {:sourceLine 70} (true);
-StateEnum_SimpleMarketplace[this] := 0;
+assert {:first} {:sourceFile "/Users/etorres/Proyectos/verisol-test/2/new_folder4/CombinationsTemp4.sol"} {:sourceLine 71} (true);
+assume (false);
+}
+assert {:first} {:sourceFile "/Users/etorres/Proyectos/verisol-test/2/new_folder4/CombinationsTemp4.sol"} {:sourceLine 74} (true);
+InstanceBuyer_AssetTransfer[this] := msgsender_MSG;
+call  {:cexpr "InstanceBuyer"} boogie_si_record_sol2Bpl_ref(InstanceBuyer_AssetTransfer[this]);
+assert {:first} {:sourceFile "/Users/etorres/Proyectos/verisol-test/2/new_folder4/CombinationsTemp4.sol"} {:sourceLine 75} (true);
+InstanceInspector_AssetTransfer[this] := inspector_s318;
+call  {:cexpr "InstanceInspector"} boogie_si_record_sol2Bpl_ref(InstanceInspector_AssetTransfer[this]);
+assert {:first} {:sourceFile "/Users/etorres/Proyectos/verisol-test/2/new_folder4/CombinationsTemp4.sol"} {:sourceLine 76} (true);
+InstanceAppraiser_AssetTransfer[this] := appraiser_s318;
+call  {:cexpr "InstanceAppraiser"} boogie_si_record_sol2Bpl_ref(InstanceAppraiser_AssetTransfer[this]);
+assert {:first} {:sourceFile "/Users/etorres/Proyectos/verisol-test/2/new_folder4/CombinationsTemp4.sol"} {:sourceLine 77} (true);
+assume ((OfferPrice_AssetTransfer[this]) >= (0));
+assume ((offerPrice_s318) >= (0));
+OfferPrice_AssetTransfer[this] := offerPrice_s318;
+call  {:cexpr "OfferPrice"} boogie_si_record_sol2Bpl_int(OfferPrice_AssetTransfer[this]);
+assert {:first} {:sourceFile "/Users/etorres/Proyectos/verisol-test/2/new_folder4/CombinationsTemp4.sol"} {:sourceLine 78} (true);
+State_AssetTransfer[this] := 1;
 }
 
-procedure {:public} {:inline 1} AcceptOffer_SimpleMarketplace(this: Ref, msgsender_MSG: Ref, msgvalue_MSG: int);
-implementation AcceptOffer_SimpleMarketplace(this: Ref, msgsender_MSG: Ref, msgvalue_MSG: int)
+procedure {:public} {:inline 1} AcceptOffer_AssetTransfer(this: Ref, msgsender_MSG: Ref, msgvalue_MSG: int);
+implementation AcceptOffer_AssetTransfer(this: Ref, msgsender_MSG: Ref, msgvalue_MSG: int)
 {
 call  {:cexpr "_verisolFirstArg"} boogie_si_record_sol2Bpl_bool(false);
 call  {:cexpr "this"} boogie_si_record_sol2Bpl_ref(this);
 call  {:cexpr "msg.sender"} boogie_si_record_sol2Bpl_ref(msgsender_MSG);
 call  {:cexpr "msg.value"} boogie_si_record_sol2Bpl_int(msgvalue_MSG);
 call  {:cexpr "_verisolLastArg"} boogie_si_record_sol2Bpl_bool(true);
-assert {:first} {:sourceFile "/Users/etorres/Proyectos/verisol-test/2/new_folder4/CombinationsTemp4.sol"} {:sourceLine 74} (true);
-assert {:first} {:sourceFile "/Users/etorres/Proyectos/verisol-test/2/new_folder4/CombinationsTemp4.sol"} {:sourceLine 75} (true);
-if ((StateEnum_SimpleMarketplace[this]) != (1)) {
-assert {:first} {:sourceFile "/Users/etorres/Proyectos/verisol-test/2/new_folder4/CombinationsTemp4.sol"} {:sourceLine 76} (true);
-assert {:first} {:sourceFile "/Users/etorres/Proyectos/verisol-test/2/new_folder4/CombinationsTemp4.sol"} {:sourceLine 77} (true);
-assume (false);
-}
-assert {:first} {:sourceFile "/Users/etorres/Proyectos/verisol-test/2/new_folder4/CombinationsTemp4.sol"} {:sourceLine 80} (true);
-if ((msgsender_MSG) != (InstanceOwner_SimpleMarketplace[this])) {
-assert {:first} {:sourceFile "/Users/etorres/Proyectos/verisol-test/2/new_folder4/CombinationsTemp4.sol"} {:sourceLine 81} (true);
-assert {:first} {:sourceFile "/Users/etorres/Proyectos/verisol-test/2/new_folder4/CombinationsTemp4.sol"} {:sourceLine 82} (true);
-assume (false);
-}
+assert {:first} {:sourceFile "/Users/etorres/Proyectos/verisol-test/2/new_folder4/CombinationsTemp4.sol"} {:sourceLine 83} (true);
+assert {:first} {:sourceFile "/Users/etorres/Proyectos/verisol-test/2/new_folder4/CombinationsTemp4.sol"} {:sourceLine 84} (true);
+if ((State_AssetTransfer[this]) != (1)) {
 assert {:first} {:sourceFile "/Users/etorres/Proyectos/verisol-test/2/new_folder4/CombinationsTemp4.sol"} {:sourceLine 85} (true);
-StateEnum_SimpleMarketplace[this] := 2;
+assert {:first} {:sourceFile "/Users/etorres/Proyectos/verisol-test/2/new_folder4/CombinationsTemp4.sol"} {:sourceLine 86} (true);
+assume (false);
+}
+assert {:first} {:sourceFile "/Users/etorres/Proyectos/verisol-test/2/new_folder4/CombinationsTemp4.sol"} {:sourceLine 88} (true);
+if ((InstanceOwner_AssetTransfer[this]) != (msgsender_MSG)) {
+assert {:first} {:sourceFile "/Users/etorres/Proyectos/verisol-test/2/new_folder4/CombinationsTemp4.sol"} {:sourceLine 89} (true);
+assert {:first} {:sourceFile "/Users/etorres/Proyectos/verisol-test/2/new_folder4/CombinationsTemp4.sol"} {:sourceLine 90} (true);
+assume (false);
+}
+assert {:first} {:sourceFile "/Users/etorres/Proyectos/verisol-test/2/new_folder4/CombinationsTemp4.sol"} {:sourceLine 93} (true);
+State_AssetTransfer[this] := 2;
+}
+
+procedure {:public} {:inline 1} Reject_AssetTransfer(this: Ref, msgsender_MSG: Ref, msgvalue_MSG: int);
+implementation Reject_AssetTransfer(this: Ref, msgsender_MSG: Ref, msgvalue_MSG: int)
+{
+var __var_3: Ref;
+call  {:cexpr "_verisolFirstArg"} boogie_si_record_sol2Bpl_bool(false);
+call  {:cexpr "this"} boogie_si_record_sol2Bpl_ref(this);
+call  {:cexpr "msg.sender"} boogie_si_record_sol2Bpl_ref(msgsender_MSG);
+call  {:cexpr "msg.value"} boogie_si_record_sol2Bpl_int(msgvalue_MSG);
+call  {:cexpr "_verisolLastArg"} boogie_si_record_sol2Bpl_bool(true);
+assert {:first} {:sourceFile "/Users/etorres/Proyectos/verisol-test/2/new_folder4/CombinationsTemp4.sol"} {:sourceLine 98} (true);
+assert {:first} {:sourceFile "/Users/etorres/Proyectos/verisol-test/2/new_folder4/CombinationsTemp4.sol"} {:sourceLine 99} (true);
+if (((((((State_AssetTransfer[this]) != (1)) && ((State_AssetTransfer[this]) != (2))) && ((State_AssetTransfer[this]) != (3))) && ((State_AssetTransfer[this]) != (4))) && ((State_AssetTransfer[this]) != (5))) && ((State_AssetTransfer[this]) != (6))) {
+assert {:first} {:sourceFile "/Users/etorres/Proyectos/verisol-test/2/new_folder4/CombinationsTemp4.sol"} {:sourceLine 100} (true);
+assert {:first} {:sourceFile "/Users/etorres/Proyectos/verisol-test/2/new_folder4/CombinationsTemp4.sol"} {:sourceLine 101} (true);
+assume (false);
+}
+assert {:first} {:sourceFile "/Users/etorres/Proyectos/verisol-test/2/new_folder4/CombinationsTemp4.sol"} {:sourceLine 103} (true);
+if ((InstanceOwner_AssetTransfer[this]) != (msgsender_MSG)) {
+assert {:first} {:sourceFile "/Users/etorres/Proyectos/verisol-test/2/new_folder4/CombinationsTemp4.sol"} {:sourceLine 104} (true);
+assert {:first} {:sourceFile "/Users/etorres/Proyectos/verisol-test/2/new_folder4/CombinationsTemp4.sol"} {:sourceLine 105} (true);
+assume (false);
+}
+assert {:first} {:sourceFile "/Users/etorres/Proyectos/verisol-test/2/new_folder4/CombinationsTemp4.sol"} {:sourceLine 108} (true);
+__var_3 := null;
+InstanceBuyer_AssetTransfer[this] := __var_3;
+call  {:cexpr "InstanceBuyer"} boogie_si_record_sol2Bpl_ref(InstanceBuyer_AssetTransfer[this]);
+assert {:first} {:sourceFile "/Users/etorres/Proyectos/verisol-test/2/new_folder4/CombinationsTemp4.sol"} {:sourceLine 109} (true);
+State_AssetTransfer[this] := 0;
+}
+
+procedure {:public} {:inline 1} Accept_AssetTransfer(this: Ref, msgsender_MSG: Ref, msgvalue_MSG: int);
+implementation Accept_AssetTransfer(this: Ref, msgsender_MSG: Ref, msgvalue_MSG: int)
+{
+call  {:cexpr "_verisolFirstArg"} boogie_si_record_sol2Bpl_bool(false);
+call  {:cexpr "this"} boogie_si_record_sol2Bpl_ref(this);
+call  {:cexpr "msg.sender"} boogie_si_record_sol2Bpl_ref(msgsender_MSG);
+call  {:cexpr "msg.value"} boogie_si_record_sol2Bpl_int(msgvalue_MSG);
+call  {:cexpr "_verisolLastArg"} boogie_si_record_sol2Bpl_bool(true);
+assert {:first} {:sourceFile "/Users/etorres/Proyectos/verisol-test/2/new_folder4/CombinationsTemp4.sol"} {:sourceLine 114} (true);
+assert {:first} {:sourceFile "/Users/etorres/Proyectos/verisol-test/2/new_folder4/CombinationsTemp4.sol"} {:sourceLine 115} (true);
+if (((msgsender_MSG) != (InstanceBuyer_AssetTransfer[this])) && ((msgsender_MSG) != (InstanceOwner_AssetTransfer[this]))) {
+assert {:first} {:sourceFile "/Users/etorres/Proyectos/verisol-test/2/new_folder4/CombinationsTemp4.sol"} {:sourceLine 116} (true);
+assert {:first} {:sourceFile "/Users/etorres/Proyectos/verisol-test/2/new_folder4/CombinationsTemp4.sol"} {:sourceLine 117} (true);
+assume (false);
+}
+assert {:first} {:sourceFile "/Users/etorres/Proyectos/verisol-test/2/new_folder4/CombinationsTemp4.sol"} {:sourceLine 120} (true);
+if ((((msgsender_MSG) == (InstanceOwner_AssetTransfer[this])) && ((State_AssetTransfer[this]) != (5))) && ((State_AssetTransfer[this]) != (6))) {
+assert {:first} {:sourceFile "/Users/etorres/Proyectos/verisol-test/2/new_folder4/CombinationsTemp4.sol"} {:sourceLine 123} (true);
+assert {:first} {:sourceFile "/Users/etorres/Proyectos/verisol-test/2/new_folder4/CombinationsTemp4.sol"} {:sourceLine 124} (true);
+assume (false);
+}
+assert {:first} {:sourceFile "/Users/etorres/Proyectos/verisol-test/2/new_folder4/CombinationsTemp4.sol"} {:sourceLine 127} (true);
+if ((((msgsender_MSG) == (InstanceBuyer_AssetTransfer[this])) && ((State_AssetTransfer[this]) != (5))) && ((State_AssetTransfer[this]) != (7))) {
+assert {:first} {:sourceFile "/Users/etorres/Proyectos/verisol-test/2/new_folder4/CombinationsTemp4.sol"} {:sourceLine 130} (true);
+assert {:first} {:sourceFile "/Users/etorres/Proyectos/verisol-test/2/new_folder4/CombinationsTemp4.sol"} {:sourceLine 131} (true);
+assume (false);
+}
+assert {:first} {:sourceFile "/Users/etorres/Proyectos/verisol-test/2/new_folder4/CombinationsTemp4.sol"} {:sourceLine 134} (true);
+if ((msgsender_MSG) == (InstanceBuyer_AssetTransfer[this])) {
+assert {:first} {:sourceFile "/Users/etorres/Proyectos/verisol-test/2/new_folder4/CombinationsTemp4.sol"} {:sourceLine 135} (true);
+assert {:first} {:sourceFile "/Users/etorres/Proyectos/verisol-test/2/new_folder4/CombinationsTemp4.sol"} {:sourceLine 136} (true);
+if ((State_AssetTransfer[this]) == (5)) {
+assert {:first} {:sourceFile "/Users/etorres/Proyectos/verisol-test/2/new_folder4/CombinationsTemp4.sol"} {:sourceLine 137} (true);
+assert {:first} {:sourceFile "/Users/etorres/Proyectos/verisol-test/2/new_folder4/CombinationsTemp4.sol"} {:sourceLine 138} (true);
+State_AssetTransfer[this] := 6;
+} else {
+assert {:first} {:sourceFile "/Users/etorres/Proyectos/verisol-test/2/new_folder4/CombinationsTemp4.sol"} {:sourceLine 140} (true);
+if ((State_AssetTransfer[this]) == (7)) {
+assert {:first} {:sourceFile "/Users/etorres/Proyectos/verisol-test/2/new_folder4/CombinationsTemp4.sol"} {:sourceLine 141} (true);
+assert {:first} {:sourceFile "/Users/etorres/Proyectos/verisol-test/2/new_folder4/CombinationsTemp4.sol"} {:sourceLine 142} (true);
+State_AssetTransfer[this] := 8;
+}
+}
+} else {
+assert {:first} {:sourceFile "/Users/etorres/Proyectos/verisol-test/2/new_folder4/CombinationsTemp4.sol"} {:sourceLine 146} (true);
+assert {:first} {:sourceFile "/Users/etorres/Proyectos/verisol-test/2/new_folder4/CombinationsTemp4.sol"} {:sourceLine 147} (true);
+if ((State_AssetTransfer[this]) == (5)) {
+assert {:first} {:sourceFile "/Users/etorres/Proyectos/verisol-test/2/new_folder4/CombinationsTemp4.sol"} {:sourceLine 148} (true);
+assert {:first} {:sourceFile "/Users/etorres/Proyectos/verisol-test/2/new_folder4/CombinationsTemp4.sol"} {:sourceLine 149} (true);
+State_AssetTransfer[this] := 7;
+} else {
+assert {:first} {:sourceFile "/Users/etorres/Proyectos/verisol-test/2/new_folder4/CombinationsTemp4.sol"} {:sourceLine 151} (true);
+if ((State_AssetTransfer[this]) == (6)) {
+assert {:first} {:sourceFile "/Users/etorres/Proyectos/verisol-test/2/new_folder4/CombinationsTemp4.sol"} {:sourceLine 152} (true);
+assert {:first} {:sourceFile "/Users/etorres/Proyectos/verisol-test/2/new_folder4/CombinationsTemp4.sol"} {:sourceLine 153} (true);
+State_AssetTransfer[this] := 8;
+}
+}
+}
+}
+
+procedure {:public} {:inline 1} ModifyOffer_AssetTransfer(this: Ref, msgsender_MSG: Ref, msgvalue_MSG: int, offerPrice_s542: int);
+implementation ModifyOffer_AssetTransfer(this: Ref, msgsender_MSG: Ref, msgvalue_MSG: int, offerPrice_s542: int)
+{
+call  {:cexpr "_verisolFirstArg"} boogie_si_record_sol2Bpl_bool(false);
+call  {:cexpr "this"} boogie_si_record_sol2Bpl_ref(this);
+call  {:cexpr "msg.sender"} boogie_si_record_sol2Bpl_ref(msgsender_MSG);
+call  {:cexpr "msg.value"} boogie_si_record_sol2Bpl_int(msgvalue_MSG);
+call  {:cexpr "offerPrice"} boogie_si_record_sol2Bpl_int(offerPrice_s542);
+call  {:cexpr "_verisolLastArg"} boogie_si_record_sol2Bpl_bool(true);
+assert {:first} {:sourceFile "/Users/etorres/Proyectos/verisol-test/2/new_folder4/CombinationsTemp4.sol"} {:sourceLine 160} (true);
+assert {:first} {:sourceFile "/Users/etorres/Proyectos/verisol-test/2/new_folder4/CombinationsTemp4.sol"} {:sourceLine 161} (true);
+if ((State_AssetTransfer[this]) != (1)) {
+assert {:first} {:sourceFile "/Users/etorres/Proyectos/verisol-test/2/new_folder4/CombinationsTemp4.sol"} {:sourceLine 162} (true);
+assert {:first} {:sourceFile "/Users/etorres/Proyectos/verisol-test/2/new_folder4/CombinationsTemp4.sol"} {:sourceLine 163} (true);
+assume (false);
+}
+assert {:first} {:sourceFile "/Users/etorres/Proyectos/verisol-test/2/new_folder4/CombinationsTemp4.sol"} {:sourceLine 165} (true);
+assume ((offerPrice_s542) >= (0));
+if (((InstanceBuyer_AssetTransfer[this]) != (msgsender_MSG)) || ((offerPrice_s542) == (0))) {
+assert {:first} {:sourceFile "/Users/etorres/Proyectos/verisol-test/2/new_folder4/CombinationsTemp4.sol"} {:sourceLine 166} (true);
+assert {:first} {:sourceFile "/Users/etorres/Proyectos/verisol-test/2/new_folder4/CombinationsTemp4.sol"} {:sourceLine 167} (true);
+assume (false);
+}
+assert {:first} {:sourceFile "/Users/etorres/Proyectos/verisol-test/2/new_folder4/CombinationsTemp4.sol"} {:sourceLine 170} (true);
+assume ((OfferPrice_AssetTransfer[this]) >= (0));
+assume ((offerPrice_s542) >= (0));
+OfferPrice_AssetTransfer[this] := offerPrice_s542;
+call  {:cexpr "OfferPrice"} boogie_si_record_sol2Bpl_int(OfferPrice_AssetTransfer[this]);
+}
+
+procedure {:public} {:inline 1} RescindOffer_AssetTransfer(this: Ref, msgsender_MSG: Ref, msgvalue_MSG: int);
+implementation RescindOffer_AssetTransfer(this: Ref, msgsender_MSG: Ref, msgvalue_MSG: int)
+{
+var __var_4: Ref;
+call  {:cexpr "_verisolFirstArg"} boogie_si_record_sol2Bpl_bool(false);
+call  {:cexpr "this"} boogie_si_record_sol2Bpl_ref(this);
+call  {:cexpr "msg.sender"} boogie_si_record_sol2Bpl_ref(msgsender_MSG);
+call  {:cexpr "msg.value"} boogie_si_record_sol2Bpl_int(msgvalue_MSG);
+call  {:cexpr "_verisolLastArg"} boogie_si_record_sol2Bpl_bool(true);
+assert {:first} {:sourceFile "/Users/etorres/Proyectos/verisol-test/2/new_folder4/CombinationsTemp4.sol"} {:sourceLine 175} (true);
+assert {:first} {:sourceFile "/Users/etorres/Proyectos/verisol-test/2/new_folder4/CombinationsTemp4.sol"} {:sourceLine 176} (true);
+if (((((((State_AssetTransfer[this]) != (1)) && ((State_AssetTransfer[this]) != (2))) && ((State_AssetTransfer[this]) != (3))) && ((State_AssetTransfer[this]) != (4))) && ((State_AssetTransfer[this]) != (5))) && ((State_AssetTransfer[this]) != (7))) {
+assert {:first} {:sourceFile "/Users/etorres/Proyectos/verisol-test/2/new_folder4/CombinationsTemp4.sol"} {:sourceLine 177} (true);
+assert {:first} {:sourceFile "/Users/etorres/Proyectos/verisol-test/2/new_folder4/CombinationsTemp4.sol"} {:sourceLine 178} (true);
+assume (false);
+}
+assert {:first} {:sourceFile "/Users/etorres/Proyectos/verisol-test/2/new_folder4/CombinationsTemp4.sol"} {:sourceLine 180} (true);
+if ((InstanceBuyer_AssetTransfer[this]) != (msgsender_MSG)) {
+assert {:first} {:sourceFile "/Users/etorres/Proyectos/verisol-test/2/new_folder4/CombinationsTemp4.sol"} {:sourceLine 181} (true);
+assert {:first} {:sourceFile "/Users/etorres/Proyectos/verisol-test/2/new_folder4/CombinationsTemp4.sol"} {:sourceLine 182} (true);
+assume (false);
+}
+assert {:first} {:sourceFile "/Users/etorres/Proyectos/verisol-test/2/new_folder4/CombinationsTemp4.sol"} {:sourceLine 185} (true);
+__var_4 := null;
+InstanceBuyer_AssetTransfer[this] := __var_4;
+call  {:cexpr "InstanceBuyer"} boogie_si_record_sol2Bpl_ref(InstanceBuyer_AssetTransfer[this]);
+assert {:first} {:sourceFile "/Users/etorres/Proyectos/verisol-test/2/new_folder4/CombinationsTemp4.sol"} {:sourceLine 186} (true);
+assume ((OfferPrice_AssetTransfer[this]) >= (0));
+OfferPrice_AssetTransfer[this] := 0;
+call  {:cexpr "OfferPrice"} boogie_si_record_sol2Bpl_int(OfferPrice_AssetTransfer[this]);
+assert {:first} {:sourceFile "/Users/etorres/Proyectos/verisol-test/2/new_folder4/CombinationsTemp4.sol"} {:sourceLine 187} (true);
+State_AssetTransfer[this] := 0;
+}
+
+procedure {:public} {:inline 1} MarkAppraised_AssetTransfer(this: Ref, msgsender_MSG: Ref, msgvalue_MSG: int);
+implementation MarkAppraised_AssetTransfer(this: Ref, msgsender_MSG: Ref, msgvalue_MSG: int)
+{
+call  {:cexpr "_verisolFirstArg"} boogie_si_record_sol2Bpl_bool(false);
+call  {:cexpr "this"} boogie_si_record_sol2Bpl_ref(this);
+call  {:cexpr "msg.sender"} boogie_si_record_sol2Bpl_ref(msgsender_MSG);
+call  {:cexpr "msg.value"} boogie_si_record_sol2Bpl_int(msgvalue_MSG);
+call  {:cexpr "_verisolLastArg"} boogie_si_record_sol2Bpl_bool(true);
+assert {:first} {:sourceFile "/Users/etorres/Proyectos/verisol-test/2/new_folder4/CombinationsTemp4.sol"} {:sourceLine 192} (true);
+assert {:first} {:sourceFile "/Users/etorres/Proyectos/verisol-test/2/new_folder4/CombinationsTemp4.sol"} {:sourceLine 193} (true);
+if ((InstanceAppraiser_AssetTransfer[this]) != (msgsender_MSG)) {
+assert {:first} {:sourceFile "/Users/etorres/Proyectos/verisol-test/2/new_folder4/CombinationsTemp4.sol"} {:sourceLine 194} (true);
+assert {:first} {:sourceFile "/Users/etorres/Proyectos/verisol-test/2/new_folder4/CombinationsTemp4.sol"} {:sourceLine 195} (true);
+assume (false);
+}
+assert {:first} {:sourceFile "/Users/etorres/Proyectos/verisol-test/2/new_folder4/CombinationsTemp4.sol"} {:sourceLine 198} (true);
+if ((State_AssetTransfer[this]) == (2)) {
+assert {:first} {:sourceFile "/Users/etorres/Proyectos/verisol-test/2/new_folder4/CombinationsTemp4.sol"} {:sourceLine 199} (true);
+assert {:first} {:sourceFile "/Users/etorres/Proyectos/verisol-test/2/new_folder4/CombinationsTemp4.sol"} {:sourceLine 200} (true);
+State_AssetTransfer[this] := 4;
+} else {
+assert {:first} {:sourceFile "/Users/etorres/Proyectos/verisol-test/2/new_folder4/CombinationsTemp4.sol"} {:sourceLine 202} (true);
+if ((State_AssetTransfer[this]) == (3)) {
+assert {:first} {:sourceFile "/Users/etorres/Proyectos/verisol-test/2/new_folder4/CombinationsTemp4.sol"} {:sourceLine 203} (true);
+assert {:first} {:sourceFile "/Users/etorres/Proyectos/verisol-test/2/new_folder4/CombinationsTemp4.sol"} {:sourceLine 204} (true);
+State_AssetTransfer[this] := 5;
+} else {
+assert {:first} {:sourceFile "/Users/etorres/Proyectos/verisol-test/2/new_folder4/CombinationsTemp4.sol"} {:sourceLine 207} (true);
+assert {:first} {:sourceFile "/Users/etorres/Proyectos/verisol-test/2/new_folder4/CombinationsTemp4.sol"} {:sourceLine 208} (true);
+assume (false);
+}
+}
+}
+
+procedure {:public} {:inline 1} MarkInspected_AssetTransfer(this: Ref, msgsender_MSG: Ref, msgvalue_MSG: int);
+implementation MarkInspected_AssetTransfer(this: Ref, msgsender_MSG: Ref, msgvalue_MSG: int)
+{
+call  {:cexpr "_verisolFirstArg"} boogie_si_record_sol2Bpl_bool(false);
+call  {:cexpr "this"} boogie_si_record_sol2Bpl_ref(this);
+call  {:cexpr "msg.sender"} boogie_si_record_sol2Bpl_ref(msgsender_MSG);
+call  {:cexpr "msg.value"} boogie_si_record_sol2Bpl_int(msgvalue_MSG);
+call  {:cexpr "_verisolLastArg"} boogie_si_record_sol2Bpl_bool(true);
+assert {:first} {:sourceFile "/Users/etorres/Proyectos/verisol-test/2/new_folder4/CombinationsTemp4.sol"} {:sourceLine 214} (true);
+assert {:first} {:sourceFile "/Users/etorres/Proyectos/verisol-test/2/new_folder4/CombinationsTemp4.sol"} {:sourceLine 215} (true);
+if ((InstanceInspector_AssetTransfer[this]) != (msgsender_MSG)) {
+assert {:first} {:sourceFile "/Users/etorres/Proyectos/verisol-test/2/new_folder4/CombinationsTemp4.sol"} {:sourceLine 216} (true);
+assert {:first} {:sourceFile "/Users/etorres/Proyectos/verisol-test/2/new_folder4/CombinationsTemp4.sol"} {:sourceLine 217} (true);
+assume (false);
+}
+assert {:first} {:sourceFile "/Users/etorres/Proyectos/verisol-test/2/new_folder4/CombinationsTemp4.sol"} {:sourceLine 220} (true);
+if ((State_AssetTransfer[this]) == (2)) {
+assert {:first} {:sourceFile "/Users/etorres/Proyectos/verisol-test/2/new_folder4/CombinationsTemp4.sol"} {:sourceLine 221} (true);
+assert {:first} {:sourceFile "/Users/etorres/Proyectos/verisol-test/2/new_folder4/CombinationsTemp4.sol"} {:sourceLine 222} (true);
+State_AssetTransfer[this] := 3;
+} else {
+assert {:first} {:sourceFile "/Users/etorres/Proyectos/verisol-test/2/new_folder4/CombinationsTemp4.sol"} {:sourceLine 224} (true);
+if ((State_AssetTransfer[this]) == (4)) {
+assert {:first} {:sourceFile "/Users/etorres/Proyectos/verisol-test/2/new_folder4/CombinationsTemp4.sol"} {:sourceLine 225} (true);
+assert {:first} {:sourceFile "/Users/etorres/Proyectos/verisol-test/2/new_folder4/CombinationsTemp4.sol"} {:sourceLine 226} (true);
+State_AssetTransfer[this] := 5;
+} else {
+assert {:first} {:sourceFile "/Users/etorres/Proyectos/verisol-test/2/new_folder4/CombinationsTemp4.sol"} {:sourceLine 229} (true);
+assert {:first} {:sourceFile "/Users/etorres/Proyectos/verisol-test/2/new_folder4/CombinationsTemp4.sol"} {:sourceLine 230} (true);
+assume (false);
+}
+}
 }
 
 procedure {:inline 1} FallbackDispatch(from: Ref, to: Ref, amount: int);
 implementation FallbackDispatch(from: Ref, to: Ref, amount: int)
 {
-if ((DType[to]) == (SimpleMarketplace)) {
+if ((DType[to]) == (AssetTransfer)) {
 assume ((amount) == (0));
 } else {
 call Fallback_UnknownType(from, to, amount);
@@ -252,117 +516,204 @@ success := false;
 }
 }
 
-const {:existential true} HoudiniB1_SimpleMarketplace: bool;
-const {:existential true} HoudiniB2_SimpleMarketplace: bool;
-const {:existential true} HoudiniB3_SimpleMarketplace: bool;
-const {:existential true} HoudiniB4_SimpleMarketplace: bool;
-const {:existential true} HoudiniB5_SimpleMarketplace: bool;
-const {:existential true} HoudiniB6_SimpleMarketplace: bool;
-procedure BoogieEntry_SimpleMarketplace();
-implementation BoogieEntry_SimpleMarketplace()
+const {:existential true} HoudiniB1_AssetTransfer: bool;
+const {:existential true} HoudiniB2_AssetTransfer: bool;
+const {:existential true} HoudiniB3_AssetTransfer: bool;
+const {:existential true} HoudiniB4_AssetTransfer: bool;
+const {:existential true} HoudiniB5_AssetTransfer: bool;
+const {:existential true} HoudiniB6_AssetTransfer: bool;
+const {:existential true} HoudiniB7_AssetTransfer: bool;
+const {:existential true} HoudiniB8_AssetTransfer: bool;
+const {:existential true} HoudiniB9_AssetTransfer: bool;
+const {:existential true} HoudiniB10_AssetTransfer: bool;
+const {:existential true} HoudiniB11_AssetTransfer: bool;
+const {:existential true} HoudiniB12_AssetTransfer: bool;
+const {:existential true} HoudiniB13_AssetTransfer: bool;
+const {:existential true} HoudiniB14_AssetTransfer: bool;
+const {:existential true} HoudiniB15_AssetTransfer: bool;
+const {:existential true} HoudiniB16_AssetTransfer: bool;
+const {:existential true} HoudiniB17_AssetTransfer: bool;
+const {:existential true} HoudiniB18_AssetTransfer: bool;
+const {:existential true} HoudiniB19_AssetTransfer: bool;
+const {:existential true} HoudiniB20_AssetTransfer: bool;
+procedure BoogieEntry_AssetTransfer();
+implementation BoogieEntry_AssetTransfer()
 {
 var this: Ref;
 var msgsender_MSG: Ref;
 var msgvalue_MSG: int;
 var choice: int;
-var offerPrice_s31: int;
-var description_s78: int;
-var price_s78: int;
-var sender_s78: Ref;
-var offerPrice_s124: int;
+var offerPrice_s143: int;
+var inspector_s143: Ref;
+var appraiser_s143: Ref;
+var description_s143: int;
+var price_s143: int;
+var description_s196: int;
+var price_s196: int;
+var description_s248: int;
+var price_s248: int;
+var inspector_s318: Ref;
+var appraiser_s318: Ref;
+var offerPrice_s318: int;
+var offerPrice_s542: int;
 var tmpNow: int;
 assume ((now) >= (0));
-assume ((DType[this]) == (SimpleMarketplace));
-call SimpleMarketplace_SimpleMarketplace(this, msgsender_MSG, msgvalue_MSG, description_s78, price_s78, sender_s78);
+assume ((DType[this]) == (AssetTransfer));
+call AssetTransfer_AssetTransfer(this, msgsender_MSG, msgvalue_MSG, description_s196, price_s196);
 while (true)
-  invariant (HoudiniB1_SimpleMarketplace) ==> ((InstanceOwner_SimpleMarketplace[this]) == (null));
-  invariant (HoudiniB2_SimpleMarketplace) ==> ((InstanceOwner_SimpleMarketplace[this]) != (null));
-  invariant (HoudiniB3_SimpleMarketplace) ==> ((InstanceBuyer_SimpleMarketplace[this]) == (null));
-  invariant (HoudiniB4_SimpleMarketplace) ==> ((InstanceBuyer_SimpleMarketplace[this]) != (null));
-  invariant (HoudiniB5_SimpleMarketplace) ==> ((InstanceOwner_SimpleMarketplace[this]) == (InstanceBuyer_SimpleMarketplace[this]));
-  invariant (HoudiniB6_SimpleMarketplace) ==> ((InstanceOwner_SimpleMarketplace[this]) != (InstanceBuyer_SimpleMarketplace[this]));
+  invariant (HoudiniB1_AssetTransfer) ==> ((InstanceOwner_AssetTransfer[this]) == (null));
+  invariant (HoudiniB2_AssetTransfer) ==> ((InstanceOwner_AssetTransfer[this]) != (null));
+  invariant (HoudiniB3_AssetTransfer) ==> ((InstanceBuyer_AssetTransfer[this]) == (null));
+  invariant (HoudiniB4_AssetTransfer) ==> ((InstanceBuyer_AssetTransfer[this]) != (null));
+  invariant (HoudiniB5_AssetTransfer) ==> ((InstanceInspector_AssetTransfer[this]) == (null));
+  invariant (HoudiniB6_AssetTransfer) ==> ((InstanceInspector_AssetTransfer[this]) != (null));
+  invariant (HoudiniB7_AssetTransfer) ==> ((InstanceAppraiser_AssetTransfer[this]) == (null));
+  invariant (HoudiniB8_AssetTransfer) ==> ((InstanceAppraiser_AssetTransfer[this]) != (null));
+  invariant (HoudiniB9_AssetTransfer) ==> ((InstanceOwner_AssetTransfer[this]) == (InstanceBuyer_AssetTransfer[this]));
+  invariant (HoudiniB10_AssetTransfer) ==> ((InstanceOwner_AssetTransfer[this]) != (InstanceBuyer_AssetTransfer[this]));
+  invariant (HoudiniB11_AssetTransfer) ==> ((InstanceOwner_AssetTransfer[this]) == (InstanceInspector_AssetTransfer[this]));
+  invariant (HoudiniB12_AssetTransfer) ==> ((InstanceOwner_AssetTransfer[this]) != (InstanceInspector_AssetTransfer[this]));
+  invariant (HoudiniB13_AssetTransfer) ==> ((InstanceOwner_AssetTransfer[this]) == (InstanceAppraiser_AssetTransfer[this]));
+  invariant (HoudiniB14_AssetTransfer) ==> ((InstanceOwner_AssetTransfer[this]) != (InstanceAppraiser_AssetTransfer[this]));
+  invariant (HoudiniB15_AssetTransfer) ==> ((InstanceBuyer_AssetTransfer[this]) == (InstanceInspector_AssetTransfer[this]));
+  invariant (HoudiniB16_AssetTransfer) ==> ((InstanceBuyer_AssetTransfer[this]) != (InstanceInspector_AssetTransfer[this]));
+  invariant (HoudiniB17_AssetTransfer) ==> ((InstanceBuyer_AssetTransfer[this]) == (InstanceAppraiser_AssetTransfer[this]));
+  invariant (HoudiniB18_AssetTransfer) ==> ((InstanceBuyer_AssetTransfer[this]) != (InstanceAppraiser_AssetTransfer[this]));
+  invariant (HoudiniB19_AssetTransfer) ==> ((InstanceInspector_AssetTransfer[this]) == (InstanceAppraiser_AssetTransfer[this]));
+  invariant (HoudiniB20_AssetTransfer) ==> ((InstanceInspector_AssetTransfer[this]) != (InstanceAppraiser_AssetTransfer[this]));
 {
 havoc msgsender_MSG;
 havoc msgvalue_MSG;
 havoc choice;
-havoc offerPrice_s31;
-havoc description_s78;
-havoc price_s78;
-havoc sender_s78;
-havoc offerPrice_s124;
+havoc offerPrice_s143;
+havoc inspector_s143;
+havoc appraiser_s143;
+havoc description_s143;
+havoc price_s143;
+havoc description_s196;
+havoc price_s196;
+havoc description_s248;
+havoc price_s248;
+havoc inspector_s318;
+havoc appraiser_s318;
+havoc offerPrice_s318;
+havoc offerPrice_s542;
 havoc tmpNow;
 tmpNow := now;
 havoc now;
 assume ((now) > (tmpNow));
 assume ((msgsender_MSG) != (null));
-assume ((DType[msgsender_MSG]) != (SimpleMarketplace));
+assume ((DType[msgsender_MSG]) != (AssetTransfer));
 Alloc[msgsender_MSG] := true;
-if ((choice) == (4)) {
-call prueba_SimpleMarketplace(this, msgsender_MSG, msgvalue_MSG, offerPrice_s31);
+if ((choice) == (11)) {
+call prueba_AssetTransfer(this, msgsender_MSG, msgvalue_MSG, offerPrice_s143, inspector_s143, appraiser_s143, description_s143, price_s143);
+} else if ((choice) == (10)) {
+call Terminate_AssetTransfer(this, msgsender_MSG, msgvalue_MSG);
+} else if ((choice) == (9)) {
+call Modify_AssetTransfer(this, msgsender_MSG, msgvalue_MSG, description_s248, price_s248);
+} else if ((choice) == (8)) {
+call MakeOffer_AssetTransfer(this, msgsender_MSG, msgvalue_MSG, inspector_s318, appraiser_s318, offerPrice_s318);
+} else if ((choice) == (7)) {
+call AcceptOffer_AssetTransfer(this, msgsender_MSG, msgvalue_MSG);
+} else if ((choice) == (6)) {
+call Reject_AssetTransfer(this, msgsender_MSG, msgvalue_MSG);
+} else if ((choice) == (5)) {
+call Accept_AssetTransfer(this, msgsender_MSG, msgvalue_MSG);
+} else if ((choice) == (4)) {
+call ModifyOffer_AssetTransfer(this, msgsender_MSG, msgvalue_MSG, offerPrice_s542);
 } else if ((choice) == (3)) {
-call MakeOffer_SimpleMarketplace(this, msgsender_MSG, msgvalue_MSG, offerPrice_s124);
+call RescindOffer_AssetTransfer(this, msgsender_MSG, msgvalue_MSG);
 } else if ((choice) == (2)) {
-call Reject_SimpleMarketplace(this, msgsender_MSG, msgvalue_MSG);
+call MarkAppraised_AssetTransfer(this, msgsender_MSG, msgvalue_MSG);
 } else if ((choice) == (1)) {
-call AcceptOffer_SimpleMarketplace(this, msgsender_MSG, msgvalue_MSG);
+call MarkInspected_AssetTransfer(this, msgsender_MSG, msgvalue_MSG);
 }
 }
 }
 
-procedure CorralChoice_SimpleMarketplace(this: Ref);
-implementation CorralChoice_SimpleMarketplace(this: Ref)
+procedure CorralChoice_AssetTransfer(this: Ref);
+implementation CorralChoice_AssetTransfer(this: Ref)
 {
 var msgsender_MSG: Ref;
 var msgvalue_MSG: int;
 var choice: int;
-var offerPrice_s31: int;
-var description_s78: int;
-var price_s78: int;
-var sender_s78: Ref;
-var offerPrice_s124: int;
+var offerPrice_s143: int;
+var inspector_s143: Ref;
+var appraiser_s143: Ref;
+var description_s143: int;
+var price_s143: int;
+var description_s196: int;
+var price_s196: int;
+var description_s248: int;
+var price_s248: int;
+var inspector_s318: Ref;
+var appraiser_s318: Ref;
+var offerPrice_s318: int;
+var offerPrice_s542: int;
 var tmpNow: int;
 havoc msgsender_MSG;
 havoc msgvalue_MSG;
 havoc choice;
-havoc offerPrice_s31;
-havoc description_s78;
-havoc price_s78;
-havoc sender_s78;
-havoc offerPrice_s124;
+havoc offerPrice_s143;
+havoc inspector_s143;
+havoc appraiser_s143;
+havoc description_s143;
+havoc price_s143;
+havoc description_s196;
+havoc price_s196;
+havoc description_s248;
+havoc price_s248;
+havoc inspector_s318;
+havoc appraiser_s318;
+havoc offerPrice_s318;
+havoc offerPrice_s542;
 havoc tmpNow;
 tmpNow := now;
 havoc now;
 assume ((now) > (tmpNow));
 assume ((msgsender_MSG) != (null));
-assume ((DType[msgsender_MSG]) != (SimpleMarketplace));
+assume ((DType[msgsender_MSG]) != (AssetTransfer));
 Alloc[msgsender_MSG] := true;
-if ((choice) == (4)) {
-call prueba_SimpleMarketplace(this, msgsender_MSG, msgvalue_MSG, offerPrice_s31);
+if ((choice) == (11)) {
+call prueba_AssetTransfer(this, msgsender_MSG, msgvalue_MSG, offerPrice_s143, inspector_s143, appraiser_s143, description_s143, price_s143);
+} else if ((choice) == (10)) {
+call Terminate_AssetTransfer(this, msgsender_MSG, msgvalue_MSG);
+} else if ((choice) == (9)) {
+call Modify_AssetTransfer(this, msgsender_MSG, msgvalue_MSG, description_s248, price_s248);
+} else if ((choice) == (8)) {
+call MakeOffer_AssetTransfer(this, msgsender_MSG, msgvalue_MSG, inspector_s318, appraiser_s318, offerPrice_s318);
+} else if ((choice) == (7)) {
+call AcceptOffer_AssetTransfer(this, msgsender_MSG, msgvalue_MSG);
+} else if ((choice) == (6)) {
+call Reject_AssetTransfer(this, msgsender_MSG, msgvalue_MSG);
+} else if ((choice) == (5)) {
+call Accept_AssetTransfer(this, msgsender_MSG, msgvalue_MSG);
+} else if ((choice) == (4)) {
+call ModifyOffer_AssetTransfer(this, msgsender_MSG, msgvalue_MSG, offerPrice_s542);
 } else if ((choice) == (3)) {
-call MakeOffer_SimpleMarketplace(this, msgsender_MSG, msgvalue_MSG, offerPrice_s124);
+call RescindOffer_AssetTransfer(this, msgsender_MSG, msgvalue_MSG);
 } else if ((choice) == (2)) {
-call Reject_SimpleMarketplace(this, msgsender_MSG, msgvalue_MSG);
+call MarkAppraised_AssetTransfer(this, msgsender_MSG, msgvalue_MSG);
 } else if ((choice) == (1)) {
-call AcceptOffer_SimpleMarketplace(this, msgsender_MSG, msgvalue_MSG);
+call MarkInspected_AssetTransfer(this, msgsender_MSG, msgvalue_MSG);
 }
 }
 
-procedure CorralEntry_SimpleMarketplace();
-implementation CorralEntry_SimpleMarketplace()
+procedure CorralEntry_AssetTransfer();
+implementation CorralEntry_AssetTransfer()
 {
 var this: Ref;
 var msgsender_MSG: Ref;
 var msgvalue_MSG: int;
-var description_s78: int;
-var price_s78: int;
-var sender_s78: Ref;
+var description_s196: int;
+var price_s196: int;
 call this := FreshRefGenerator();
 assume ((now) >= (0));
-assume ((DType[this]) == (SimpleMarketplace));
-call SimpleMarketplace_SimpleMarketplace(this, msgsender_MSG, msgvalue_MSG, description_s78, price_s78, sender_s78);
+assume ((DType[this]) == (AssetTransfer));
+call AssetTransfer_AssetTransfer(this, msgsender_MSG, msgvalue_MSG, description_s196, price_s196);
 while (true)
 {
-call CorralChoice_SimpleMarketplace(this);
+call CorralChoice_AssetTransfer(this);
 }
 }
 
